Release of coq-smartcontracts

Auction/Auction.sol
@@ -1,0 +1,30 @@
+contract Auction {
+    int public highestBid;
+
+    mapping (address => bool) public isWinner; 
+    mapping (address => int) public bids;
+
+    function Auction (){
+        highestBid = 0;
+        isWinner[msg.sender] = true;
+    }
+
+    function bid(int value) {
+        if (bids[msg.sender] > value) throw;
+        else {
+            bids[msg.sender] = value;
+            if (value > highestBid) {
+                highestBid = value;
+                isWinner[msg.sender] = true;
+            }
+        }
+    }
+
+    function get_money() {
+        if (isWinner[msg.sender]) {
+            msg.sender.send(highestBid);
+            isWinner[msg.sender] = false;
+        }
+    }
+        
+}
