Ballot/Ballot.sol
@@ -1,0 +1,45 @@
+contract Ballot {
+    // Create a new ballot with $(_numProposals) different proposals.
+    function Ballot(uint8 _numProposals) {
+        chairperson = sender;
+        numProposals = _numProposals;
+    }
+
+    // Give $(voter) the right to vote on this ballot.
+    // May only be called by $(chairperson).
+    function giveRightToVote(address voter) {
+        if (/*msg.sender != chairperson ||*/ voted[voter]) return;
+        voterWeight[voter] = 1;
+    }
+
+    // Delegate your vote to the voter $(to).
+    function delegate(address to) {
+        if (voted[sender]) return;
+        if (to == sender) return;
+        voted[sender] = true;
+        delegations[sender] = to;
+        if (voted[to]) voteCounts[votes[to]] += voterWeight[sender];
+        else {voterWeight[to] += voterWeight[sender];
+             voterWeight[sender] = 0;}
+    }
+
+    // Give a single vote to proposal $(proposal).
+    function vote(uint8 proposal) {
+        if (voted[sender] || proposal >= numProposals) return;
+        voted[sender] = true;
+        votes[sender] = proposal;
+        voteCounts[proposal] += voterWeight[sender];
+    }
+
+    @preservation(voterWeight, snd(x))
+
+    address chairperson;
+    uint8 numProposals;
+    mapping(address => uint256) voterWeight;
+    mapping(address => bool) voted;
+    mapping(address => uint8) votes;
+    mapping(address => address) delegations;
+    mapping(uint8 => uint256) voteCounts;
+}
+
+
