Compiler/codegen.ml
@@ -1,0 +1,568 @@
+(** This file generates coq code directly from the modified AST 
+This code does not support the generation of several contracts, the whole code should consist of one Solidity contract
+**)
+
+open Tast
+open Lemmas
+exception Error of string
+
+(* Used to keep track of required module in Coq *)
+let required_modules = ref ["Arith"; "Nat"; "OrderedTypeEx"; "Coq.FSets.FMapList"; "BinInt"; "BinIntDef"]
+let open_string = ref false
+module VSet = Set.Make(String)
+
+(* Keeps track of all state variables of the current contract *)
+let state_vars = ref VSet.empty
+let state_list = ref ["Unused"]
+
+(* Names of functionns present reachable in the file to avoid generating events. Events should perhaps be removed in passes *)
+let fun_names = ref ["()"; "fst"; "snd"; "send"]
+
+(* Counter to generate unique auxiliary functions to model loops *)
+let count_while = ref 0
+(* The following references are used to store the auxiliary functions for loops, and the structures for passing and getting values from these functions, 
+in order to generate them before any other function to avoid dependency issues *)
+let while_structs = ref ""
+let while_functions = ref ""
+
+(* Helper to indicate that a Coq module is required *)
+let add_required m = 
+    if not (List.mem m (!required_modules)) then required_modules := m::(!required_modules)
+
+(* Print the list of names of state variables *)
+let rec print_state_vars = function
+    | [] -> ""
+    | a::q -> " "^a^(print_state_vars q)
+
+(* Generates the type of a Solidity mapping in Coq, to declare a variable *)
+let rec generate_mapping (e : Tast.elem_type_name) (t : Tast.type_name) = (match e with
+    | TEInt | TEAddress -> "IntMap.t (" ^ (generate_type t) ^ ")"
+    | TEString -> raise (Error ("string as map keys not supported")) 
+    | TEBool -> raise (Error ("bool as map keys not supported"))
+    )
+    
+(* Generates elementary types in Coq *)
+and generate_elem_type = function
+    | TEInt -> "Z"
+    | TEString -> add_required "String"; "string"
+    | TEAddress -> "Z"
+    | TEBool -> "bool"
+
+(* Generates a type in Coq *)
+and generate_type (t : Tast.type_name) = match t with
+    | TIdent id -> id
+    | TElem e -> generate_elem_type e
+    | TMapping (e, t) -> generate_mapping e t
+
+(* Creates a default value for a mapping. Default value means that the mapping is empty *)
+let rec init_mapping (e : Tast.elem_type_name) (t : Tast.type_name) = (match e with
+    | TEInt | TEAddress -> "IntMap.empty (" ^ (generate_type t) ^ ")"
+    | TEString -> raise (Error ("string as map keys not supported")) 
+    | TEBool -> raise (Error ("bool as map keys not supported"))
+    )
+
+(* Generates a list of expressions *)
+let rec generate_expression_list name = function
+    | [] -> ""
+    | a::q -> " (" ^ (generate_expression a name) ^ ")" ^ (generate_expression_list name q)
+
+(* Generates expressions for the AST.
+For a function call, we decrease the amount of gas before passing the new gas value, all the state variables, 
+the ether balance of all accounts, the message from the sender, and finally all the parameters of the function. **)
+and generate_expression (e : Tast.expression) name = match e with
+    | EInt i -> string_of_int i 
+    | EBool b -> string_of_bool b 
+    | EStr s -> add_required "String"; open_string := true; "\"" ^s ^ "\"" 
+    | EVar id -> id 
+    | EFieldVar (e, id) -> (match e with
+        | EVar ("msg") -> if (id = "sender") then "(sender msg)" else 
+            if (id = "value") then "(value msg)" else raise (Error ("only msg.sender, msg.value and msg.gas supported for msg object")) 
+        | _ -> raise (Error "EFieldVar not supported")) (* "(" ^ id ^ " " ^ (generate_expression e) ^ ")" ) *)
+    | EArrayVar (id, el) -> "(get_"^id^ " " ^ id ^" " ^(generate_expression_list name el) ^")"
+    | EConditional (e1, e2, e3) -> "if ("^(generate_expression e1 name) ^ ") then (" ^ (generate_expression e2 name) ^")\n else ("^(generate_expression e3 name) ^ ")\n" 
+    | ENot e -> "( xorb  " ^ (generate_expression e name) ^" true)" 
+    | EInc e -> raise (Error "Inc expression not supported yet") 
+    | EDec e -> raise (Error "Dec expression not supported yet")
+    | EBinOp (op, e1, e2) -> (match op with
+        | OpLt -> "( ltb " ^ (generate_expression e1 name) ^ " "^ (generate_expression e2 name) ^")"
+        | OpLe -> "( leb " ^ (generate_expression e1 name) ^ " "^ (generate_expression e2 name) ^")"
+        | OpGt -> "( leb " ^ (generate_expression e2 name) ^ " "^ (generate_expression e1 name) ^")"
+        | OpGe -> "( ltb " ^ (generate_expression e2 name) ^ " "^ (generate_expression e1 name) ^")"
+        | OpEq -> "( eqb " ^ (generate_expression e1 name) ^ " "^ (generate_expression e2 name) ^ ")"
+        | OpNeq -> "( xorb ( eqb " ^ (generate_expression e1 name) ^ " "^ (generate_expression e2 name) ^") true )"
+        | OpPlus -> "(" ^ (generate_expression e1 name) ^ " + " ^ (generate_expression e2 name) ^ ")"
+        | OpMinus -> "(" ^ (generate_expression e1 name) ^ " - " ^ (generate_expression e2 name) ^ ")"
+        | OpMul -> "(" ^ (generate_expression e1 name) ^ " * " ^ (generate_expression e2 name) ^ ")"
+        | OpAnd -> "( andb " ^ (generate_expression e1 name) ^ " " ^ (generate_expression e2 name) ^ ")"
+        | OpOr -> "( orb " ^ (generate_expression e1 name) ^ " " ^ (generate_expression e2 name) ^ ")"
+        )        
+    | EFunCall (id, el) -> if (List.mem id (!fun_names)) then "let new_gas := (Nat.pred new_gas) in\n (" ^ id ^ " new_gas (create_"^name ^ (print_state_vars (List.tl(List.rev((!state_list))))) ^ ") new_ether msg" ^ (generate_expression_list name el) ^ ")" else ""
+    | EFieldFunCall (e, id, el) -> raise (Error "FieldFunCall expression not supported yet")
+
+(* Helper to generate expressions when an Option structure is involved *)
+let generate_expression_opt ( eo : Tast.expression option) name =
+    match eo with
+    | None -> ""
+    | Some e -> " := " ^ (generate_expression e name)
+
+(* Declares a field of a structure. Used recursively to declare a structure *)
+let generate_struct_var (v : Tast.variable_def) name =
+    v.v_name ^ ": " ^ generate_type v.v_type ^ generate_expression_opt v.v_expr name ^ ";\n"
+
+(* Generates a structure by calling recursively generate_struct_var *)
+let rec generate_struct_vars_decl name = function
+    | [] -> ""
+    | a::q -> generate_struct_var a name ^ generate_struct_vars_decl name q
+
+(* Helper function to generate one variable un a structure without possible initial value *)
+let generate_struct_state_var (v : Tast.variable_def) =
+    v.v_name ^ ": " ^ generate_type v.v_type ^ ";\n"
+
+(* Calls recursively generate_struct_state_var to generate a whole structure *)
+let rec generate_struct_state_vars_decl = function
+    | [] -> ""
+    | a::q -> generate_struct_state_var a ^ generate_struct_state_vars_decl q
+
+(* The global state of the contract comprises its state variables. We store and pass them as a record in Coq.
+This function generates the structure to contain all the state variables specifically *)
+let generate_state_vars (vars : Tast.variable_def list) (name : ident) =
+    List.iter (fun v -> state_list := (v.v_name)::(!state_list); state_vars := VSet.add v.v_name (!state_vars)) vars; 
+    "Record " ^ name ^" := create_"^name^" { \n" ^ (generate_struct_state_vars_decl vars) ^ "}.\n"
+
+(* Called at the beginning of each function generation to extract all the values of the state variables passed as a Record to the function *)
+let rec create_base_state_vars (vars : Tast.variable_def list) name =
+    match vars with
+    | [] -> ""
+    | a::q -> ("let " ^ a.v_name ^ " := ("^ a.v_name ^ " " ^name^") in\n") ^ (create_base_state_vars q name)
+
+(* Generate one function parameter, and specifies its Coq type *)
+let generate_param (param : Tast.type_name * ident) =
+    "(" ^ (snd param) ^ ":" ^ (generate_type (fst param)) ^ ") "
+    
+(* Generates the list of parameters of a function in its Coq prototype *)
+let rec generate_func_params (params : (Tast.type_name * ident) list) =
+    match params with
+    | [] -> ""
+    | a::q -> (generate_param a) ^ (generate_func_params q)
+
+(* Generates all the return parameters of a function given its list of return parameters from the AST *)
+let rec generate_return_par = function
+    | [] -> ""
+    | a::q-> ", "^(snd a) ^ (generate_return_par q)
+
+(* When mappings are chained, we access them in a row, and call them imap0, imap1, …
+This funtion generates the name of an intermediate map given its id *)
+let get_name_map id = function
+    | 0 -> id
+    | i -> "imap"^(string_of_int i)
+
+(* Returns the value of the element at the end of a chaining of mappings. i.e. mapping (string -> mapping (int, bool)) returns bool *)
+let rec get_final_map_type = function
+    | TIdent s -> raise (Error "Mapping of custom classes not supported")
+    | TMapping (e, t) -> get_final_map_type t
+    | TElem e -> e
+
+(* Returns a default value for a possibly chained mapping *)
+let rec base_map_nat t = function
+    | 0 -> (match get_final_map_type t with
+        | TEInt | TEAddress -> string_of_int(0)
+        | TEString -> "\"\""
+        | TEBool -> "false")
+    | i -> "IntMap.empty ("^(base_map_nat_aux t (i-1))^")"
+
+(* Returns the complete type of a possible chained mapping *)
+and base_map_nat_aux t = function
+    | 0 -> (match get_final_map_type t with
+        | TEInt | TEAddress -> "Z"
+        | TEString -> "string"
+        | TEBool -> "bool")
+    | i -> "IntMap.t ("^(base_map_nat_aux t (i-1))^")"
+
+(* Generates accessors for all the intermediate maps in a chained mapping *)
+let rec generate_intermediate_maps name id i length t= function
+    | [] -> ""
+    | a::q -> "let "^(get_name_map id (i+1))^" := match (IntMap.find "^ (generate_expression a name) ^ " " ^ (get_name_map id i) ^ ") with\n |None => "^(base_map_nat t (length-i-1)) ^"\n | Some a => a end in\n" ^ (generate_intermediate_maps name id (i+1) length t q) (* Needs some typing. Not always base_map_nat *)
+
+(* Generates an access in a possible chained mapping *)
+let rec generate_map_access id el e i name= match el with
+    | [] -> generate_expression e name
+    | a::q -> "IntMap.add " ^ (generate_expression a name) ^ " (" ^ (generate_map_access id q e (i+1) name) ^ ")" ^ (get_name_map id i)
+
+(* Generates a variable assignment *)
+let rec generate_var_assign name = function
+    | VAIdent (op, id, e) -> "let " ^id ^ " := " ^ (match op with
+        | Assign -> generate_expression e name
+        | AssignAdd -> id ^ " + " ^ (generate_expression e name)
+        | AssignSub -> id ^ " - " ^ (generate_expression e name)
+        | AssignMul -> id ^ " * " ^ (generate_expression e name)
+        ) ^" in \n"
+    | VAField (op, e1, id, e2) -> raise (Error ("VAField not implemented"))
+    | VAIdentArray (op, id, el, e, t) -> (match op with
+        | Assign -> (generate_intermediate_maps name id 0 (List.length el) t el) ^ "let "^id ^ " := " ^ (generate_map_access id el e 0 name) ^" in\n" 
+        | AssignAdd -> (generate_var_assign name (VAIdentArray(Assign, id, el, EBinOp(OpPlus, EArrayVar(id, el), e), t)))
+        | AssignSub -> (generate_var_assign name (VAIdentArray(Assign, id, el, EBinOp(OpMinus, EArrayVar(id, el), e), t)))
+        | AssignMul -> (generate_var_assign name (VAIdentArray(Assign, id, el, EBinOp(OpMul, EArrayVar(id, el), e), t)))
+        )
+    | VAFieldArray (op, e1, id, el, e2, t) -> raise (Error ("VAFieldArray not implemented"))
+
+(* Generates the complete parameters returned by a function. It consists of the record of state variables corresponding to the new global state, the new ether balances of all Ethereum users and the return values of the function itself *)
+let generate_return_params (ret_params : (Tast.type_name * ident) list) name = 
+    match ret_params with
+    | [] -> "((create_"^name ^ (print_state_vars (List.tl(List.rev((!state_list)))))^ "), new_ether)"
+    | l -> "((create_"^name ^ (print_state_vars (List.tl(List.rev(!state_list)))) ^"), new_ether"^ (generate_return_par l) ^")\n"
+
+(* Generate return values during a throw *)
+let rec generate_throw_par = function
+    | [] -> ""
+    | a::q -> ", "^(snd a) ^ (generate_throw_par q)
+
+(* Generate the complete throw parameters, including the initial global state and initial ether balances *)
+let generate_throw_return (ret_params : (Tast.type_name * ident) list) name = 
+    match ret_params with
+    | [] -> "(" ^ name ^ ", ether)"
+    | l -> "("^name ^ ", ether" ^ (generate_throw_par l) ^ ")\n"
+
+(* Helper function used during the declaration of variables. If no initial value was specified, a default one is created *)
+let generate_expr_opt_vardecl (eo : Tast.expression option) (t : Tast.type_name) name =
+    match eo with
+    | None -> (match t with
+        | TIdent id -> raise (Error ("Initialization of complex types not supported"))
+        | TMapping (e, m) -> init_mapping e m 
+        | TElem e -> (match e with
+            | TEInt | TEAddress -> "0 "
+            | TEBool -> "false "
+            | TEString -> add_required "String"; open_string := true; "\"\"")
+        )
+    | Some e -> generate_expression e name
+
+(* Generates a variable, with the specified value if there is one, with a default value if not *)
+let generate_var_decl (v : Tast.variable_def) name =
+    "let " ^v.v_name ^ " := " ^ (generate_expr_opt_vardecl v.v_expr v.v_type name) ^" in\n"
+
+(* Returns true if a list of instructions ends with a return, exception or if/then/else block *)
+let ends_with_Return l =
+    match (List.hd (List.rev l)) with
+        | SReturn _  | SThrow | SIfElse _-> true
+        | _ -> false
+
+(* Returns true if a statement or a block ends with a return *)
+let block_ends_with_return = function
+    | SBlock st -> ends_with_Return st
+    | SReturn _ | SThrow | SIfElse _ -> true
+    | _ -> false
+
+(* Returns true if a list of instructions ends with a return, exception or if/then/else block *)
+let list_ends_with_Return = function
+    | [] -> false
+    | l -> ends_with_Return l
+
+(* A loop is compiled as an auxiliary instruction. To pass the complete scope of variables, we use a Record. This function generates this structure *)
+let rec generate_while_struct = function 
+    | [] -> ""
+    | a::q -> (fst a) ^ (string_of_int (!count_while)) ^ " : " ^ (snd a) ^ ";\n" ^ generate_while_struct q
+
+(* Generates the declaration of the list of variables in scope of a loop *)
+let rec generate_while_vars i str = function
+    | [] -> ""
+    | a::q -> "let " ^ (fst a) ^ " := (" ^ (fst a) ^ (string_of_int i) ^ " "^str^ (string_of_int i) ^ ") in\n" ^ (generate_while_vars i str q)
+
+(* Prints the name of all variables in the scope of a loop *)
+let rec print_while_vars = function
+    | [] -> ""
+    | a::q -> (fst a) ^ " " ^ (print_while_vars q)
+
+(* Generates instructions inside a loop *)
+let rec generate_while_statement name = function
+    | SIf (e, st, cont) -> raise (Error ("if in while unsupported"))
+    | SIfElse (e, st1, st2, cont) -> raise (Error ("ifelse in while unsupported"))
+    | SWhile (e, s) -> raise (Error ("imbricated while not supported"))
+    | SBlock (sl) -> generate_while_statements name sl 
+    | SReturn eo -> raise (Error ("return in while not supported"))
+    | SThrow -> raise (Error ("throw in while not supported"))
+    | SExpr e -> generate_expression e name 
+    | SVarDecl v -> generate_var_decl v name 
+    | SVarAssign va -> generate_var_assign name va 
+
+(* Recursively generates the core of a loop *)
+and generate_while_statements name = function
+    | [] -> ""
+    | a::q -> (generate_while_statement name a) ^ (generate_while_statements name q)
+
+(* Completly generates the auxiliary function to model a loop. It updates the while_structs and while_functions references, to be added at the beginning of the Coq code *)
+let generate_while_auxfunction e s vars name = 
+    while_structs := (!while_structs) ^ "Record whilestruct" ^ (string_of_int (!count_while)) ^ " := create_whilestruct" ^ (string_of_int (!count_while)) ^ " {\n" ^ (generate_while_struct vars) ^ "}.\n"; 
+    while_functions := (!while_functions) ^ "Fixpoint whilefunction" ^ (string_of_int (!count_while)) ^ " (msg : Message) gas (input"^(string_of_int (!count_while))^" : whilestruct" ^ (string_of_int (!count_while)) ^ ") := \n" ^ (generate_while_vars (!count_while) "input" vars) ^ "match gas with
+    | O => (gas, create_whilestruct"^(string_of_int (!count_while)) ^ " "^ (print_while_vars vars) ^") " ^ 
+    "\n | S g => let new_gas := g in\n" ^ 
+    "if (" ^ (generate_expression e name) ^ ") then (" ^ (generate_while_statements name s) ^ "whilefunction"^ (string_of_int (!count_while)) ^ " msg new_gas (create_whilestruct"^(string_of_int (!count_while)) ^ " " ^ (print_while_vars vars) ^")) else \n" ^ "(new_gas, create_whilestruct"^(string_of_int (!count_while)) ^ " " ^ (print_while_vars vars) ^") end.\n";
+     count_while := (!count_while) + 1;
+     "let (new_gas, result"^(string_of_int ((!count_while) -1)) ^ ") := whilefunction" ^ (string_of_int ((!count_while) - 1)) ^ " msg new_gas (create_whilestruct" ^ (string_of_int ((!count_while) - 1)) ^ " " ^ (print_while_vars vars) ^ ") in\n" ^ (generate_while_vars ((!count_while) -1) "result" vars) 
+
+(* Generates a statement. An if or if/else statement has to merge the control flow after it, thus two paths are created by copying the instructions remaining after it.
+We also keep the list of variables currently in the context as *vars* to pass it to a loop auxiliary function if we need one *)
+let rec generate_statement (s : Tast.statement) ret_params name vars = match s with
+    | SIf (e, st, cont) -> "if (" ^ (generate_expression e name) ^ ") then (" ^ (generate_statement st ret_params name vars) ^ (if (block_ends_with_return st) then "" else ((generate_insns cont ret_params name vars) ^ (if list_ends_with_Return cont then  "" else generate_return_params ret_params name))) ^ ") \n else " 
+    | SIfElse (e, st1, st2, cont) -> "if (" ^ (generate_expression e name) ^ ") then (" ^ (generate_statement st1 ret_params name vars) ^ (if (block_ends_with_return st1) then "" else ((generate_insns cont ret_params name vars) ^ (if list_ends_with_Return cont then "" else generate_return_params ret_params name))) ^ ") \nelse (" ^ (generate_statement st2 ret_params name vars) ^ (if (block_ends_with_return st2) then "" else ((generate_insns cont ret_params name vars) ^ (if list_ends_with_Return cont then "" else generate_return_params ret_params name))) ^ ")\n"
+    | SWhile (e, s) -> generate_while_auxfunction e s vars name
+    | SBlock (sl) -> generate_insns sl ret_params name vars
+    | SReturn (eo) -> (match eo with 
+        | None -> generate_return_params ret_params name
+        | Some (EFunCall (id, e)) -> generate_expression (EFunCall (id, e)) name
+        | Some e -> "(create_"^name ^ (print_state_vars (List.tl(List.rev((!state_list))))) ^ ", new_ether, "^ (generate_expression e name) ^")\n"
+        )
+    | SThrow -> generate_throw_return ret_params name 
+    | SExpr e -> generate_expression e name
+    | SVarDecl v -> generate_var_decl v name 
+    | SVarAssign va -> generate_var_assign name va 
+
+(* Generates recursively the list of instructions in a function, by calling generate_statement.
+If we declare a new variable, we add it to the current context of variables *vars* to use it for the generation of loops in generate_statement *)
+and generate_insns (insns : Tast.statement list) ret_params name vars  = match insns with
+    | [] -> ""
+    | a::q -> (match a with 
+        | SIfElse _ -> (generate_statement a ret_params name vars)
+        | SVarDecl v -> (generate_statement a ret_params name vars) ^ (generate_insns q ret_params name (((v.v_name, generate_type v.v_type)::vars)))
+        | _ -> (generate_statement a ret_params name vars) ^ (generate_insns q ret_params name vars)
+    )
+
+(* Creates an initial default value for an element of type t *)
+let initialize_value (t : Tast.type_name) name =
+    match t with
+    | TIdent id -> raise (Error ("Initialization of complex types not supported in initialize_value"))
+    | TMapping (e, m) -> init_mapping e m 
+    | TElem e -> (match e with 
+            | TEInt | TEAddress -> "0"
+            | TEBool -> "false"
+            | TEString -> add_required "String"; open_string := true; "\"\""
+            )
+
+(* Generates placeholder values for all the return parameters, corresponding to the 0 representation in Solidity.
+These values are thus returned directly if the return parameters are never initialized in the Solidity code, as specified in the Solidity semantics *)
+let rec create_base_return (ret_params : (Tast.type_name * ident) list) name = 
+    match ret_params with
+        | [] -> "let new_ether := ether in \n"
+        | a::q -> "let " ^ (snd a) ^" := "^ (initialize_value (fst a) (snd a)) ^ " in \n"^ (create_base_return q name)
+
+(* For a contract constructor, values are initialized as written in the Solidity code, and the untouched values are given a 0 representation as an initial value.
+This function creates the 0 default representation for all the state variables in the Coq code of the constructor *)
+let rec create_constr_state_vars (vars : Tast.variable_def list) name = 
+    match vars with
+    | [] -> "let new_ether := ether in\n"
+    | a::q -> ("let " ^ a.v_name ^ " := "^(initialize_value a.v_type a.v_name) ^ " in\n") ^ (create_constr_state_vars q name)
+
+(* Creates a list of all parameters of a function, with the form (name : type) *)
+let rec collect_func_params = function
+    | [] -> [] 
+    | a::q -> ((snd a, generate_type (fst a)))::(collect_func_params q)
+
+(* Creates a list of all state variables of the contract, with the form (name : type) *)
+let rec collect_base_state_vars = function
+    | [] -> []
+    | a::q -> ((a.v_name, generate_type a.v_type))::(collect_base_state_vars q)
+
+(* Creates a list of all return parameters of a function, with the form (name : type) *)
+let rec collect_base_return = function
+    | [] -> []
+    | a::q -> ((snd a, generate_type (fst a)))::(collect_base_return q) 
+
+(** 
+Generation of a function: All functions are declared in Coq as recursive to be able to model a possible reentrancy.
+We distinguish between two cases: the function is the contract constructor, in this case we create a new coherent global state, and the function is not.
+We currently have a simple model of gas consumption: at each function call, we decrease by one the amount of gas. 
+If we don't have gas left, we throw an exception, and return the initial values of the input parameters. This ensures the terminaison in Coq.
+We give as input parameters of the function the amount of gas, the global state of the contract containing all state variables, the ether balances of all users,
+the message sent by an user to execute a function, and finally the actual input parameters of the function if there are any.
+We finally generate all the function statements in Coq, and add to these a return statement if the Solidity code didn't end with a return or a throw.
+**)
+let generate_function (f : Tast.function_def) name c_vars = 
+if not (f.func_insns = []) then (
+    "Fixpoint " ^ (if (name = f.func_name) then name^"_constructor" else f.func_name ^ " gas (" ^ name ^ ":" ^ name ^ ") ") ^ ("(ether : EtherMap) (msg : Message)") ^ (generate_func_params f.func_params) ^ " := \n" ^ (if (name = f.func_name) then (create_constr_state_vars c_vars name) else (create_base_state_vars c_vars name) ^ (create_base_return f.func_ret_params name)) ^ (if (name = f.func_name) then "" else "match gas with
+    | O => "^ (generate_return_params f.func_ret_params name) ^ 
+    "\n | S g => let new_gas := g in\n") ^ (generate_insns f.func_insns f.func_ret_params name (("new_ether", "EtherMap")::(collect_func_params f.func_params)@(collect_base_state_vars c_vars)@(collect_base_return f.func_ret_params))) ^ (if not (ends_with_Return f.func_insns) then (generate_return_params f.func_ret_params name) else "") ^ (if (name = f.func_name) then ".\n" else "end.\n"))
+    else ""
+
+(* Generates all the functions in the contract by recursively calling generate_function.
+c_vars is here the list of state variables of the contract, that are automatically in the context of any function *)
+let rec generate_functions (funs : Tast.function_def list) (name : ident) c_vars =
+match funs with 
+    | [] -> ""
+    | a::q -> (generate_functions q name c_vars) ^ (generate_function a name c_vars)
+    
+(* Generates structures in the contract. Not implemented yet *)
+let generate_struct_vars (sts : Tast.struct_def list) name =
+    match sts with
+        | [] -> ""
+        | a::q -> raise (Error ("struct definition not implemented"))
+
+(* Generates the anonymous "()" function of the contract. This function is called in Solidity when ether is sent to the contract. Its generation is similar to other functions *)
+let generate_anonymous_fun (insns : Tast.statement list) name =
+    if insns != [] then (
+    "Definition anonymous_function ("^ name ^ " : " ^name ^") (ether : EtherMap) (msg : Message) :=\n" ^ (create_base_return [] name) ^ (generate_insns insns [] name [("new_ether", "EtherMap")]) ^ (if not (ends_with_Return insns) then (generate_return_params [] name) else "") ^ ".\n" ) else ""
+
+
+(* Generates a default value for the last element at the end of a chain of mappings. For instance, 0 for mapping (string -> mapping (bool, int)) *)
+let rec create_base_final_value = function
+    | TMapping(e, t) -> create_base_final_value t
+    | TIdent _ -> raise (Error "map of idents not supported")
+    | TElem e -> (match e with 
+        | TEInt | TEAddress -> "0"
+        | TEBool -> "false"
+        | TEString -> "\"\""
+        )
+
+(* Helper function to generate accessors for intermediate mappings in a chain of mappings *)
+let matching_for_accessor i = function
+    | TIdent _ -> raise (Error "Ident maps not supported")
+    | TMapping (e, t) -> "| None => None \n | Some a => IntMap.find a"^(string_of_int i)^ " a"
+    | TElem t -> "| None => " ^(create_base_final_value (TElem t)) ^ "\n | Some a => a"
+
+(* Creates of an accessor for the i-th intermediate mapping *)
+let rec create_match_accessor i curr_str= function
+    | TMapping (el, t) -> "let m"^(string_of_int (i+1)) ^  ":= match "^(if (curr_str = "mapping") then  ("(IntMap.find a"^(string_of_int i) ^ " " ^ curr_str ^ ") ") else ("m"^(string_of_int i)))^ " with\n " ^ (matching_for_accessor i t) ^ " end in \n" ^ (create_match_accessor (i+1) ("m"^(string_of_int (i+1))) t)
+    | t -> "m"^(string_of_int i) 
+
+(* Generates input parameters for creating an accessor of the whole mapping *)
+let rec generate_n_ints i= function
+    | TMapping (el, t) -> "(a" ^ (string_of_int i) ^ " : Z) " ^ (generate_n_ints (i+1) t) 
+    | _ -> ""
+
+(* Maps in Coq and Solidity have a slightly different behaviour. In Solidity, if the key is not in the map, a "0" value is returned when accessing it.
+In Coq, accessing a key k returns Some a if there was something previously stored, None if not.
+We thus generate accessors for all state variables maps in the contract *)
+let rec create_accessors = function
+    | [] -> ""
+    | a::q -> (match a.v_type with
+        | TMapping _ -> "Definition get_"^a.v_name ^" (mapping : " ^ (generate_type a.v_type) ^" ) " ^ (generate_n_ints 0 a.v_type) ^ ":= \n" ^ (create_match_accessor 0 "mapping" a.v_type) ^ ".\n" ^ (create_accessors q)
+        | _ -> "")
+
+(** 
+The following functions are used to generate Coq theorems for properties written in annotations in Solidity.
+They also generate the helper lemmas corresponding to the property we are trying to prove.
+Currently, we only target preservation properties, i.e. proving that a state variable or
+an expression involving a state variable remains constant throughout any execution of the contract.
+We thus express that this quantity is preserved though the execution of any public function with any parameters
+ **)
+
+(* Retrieves the type of the variable specified in the annotation from the list of state variables *)
+let rec get_annot_var_type var = function
+    | [] -> raise (Error (var ^ " is not a state variable valid for the annotation"))
+    | a::q -> (if (a.v_name = var) then a.v_type else get_annot_var_type var q)
+
+(* Returns the list of parameters required in a lemma *)
+let rec lemma_func_params = function
+    | [] -> ""
+    | a::q -> " " ^ (snd a) ^ lemma_func_params q
+
+(** 
+Generates the list of Lemmas to prove the preservation of a property, when the variable v involved in the property has a simple type (i.e. not a mapping or an object)
+For each function f in the contract, we generate a lemma preservation_f_v that expresses that the expression with v is invariant through any execution of f.
+We finally use Admitted as placeholder to have a correct Coq code, and let the proof of the lemma to the user.
+**)
+let rec generate_simple_annot (annot : Tast.annotation_def) name = function
+    | [] -> ""
+    | a::q -> if (List.mem a.func_name annot.an_funs || (name = a.func_name)) then "" else "Lemma preservation_"^(a.func_name)^"_"^(annot.an_var)^" : forall (" ^ name ^ " : " ^ name ^ ") " ^ (generate_func_params a.func_params) ^ ", \n let " ^ name ^ "_2 := "^ 
+    (match a.func_ret_params with
+        | h::l -> " fst( " ^ (a.func_name) ^ " " ^ name ^  (lemma_func_params a.func_params) ^ ")" 
+        | [] -> (a.func_name) ^ " " ^ name ^  (lemma_func_params a.func_params) ) 
+    ^ " in\n (" ^ (annot.an_var) ^ " " ^ name ^ ") = (" ^ (annot.an_var) ^" " ^ name ^"_2)" ^ 
+    ".\nAdmitted.\n\n " ^ (generate_simple_annot annot name q)
+
+(** 
+Generates the list of Lemmas to prove the preservation of a property, when the variable v involved in the property has a mapping type
+For each function f in the contract, we generate a lemma preservation_f_v that expresses that the expression with v is invariant through any execution of f.
+The lemma generated expresses that the sum of eval(x) on all elements of the mapping, where eval is the function specified in the annotation, is preserved.
+We finally use Admitted as placeholder to have a correct Coq code, and let the proof of the lemma to the user.
+**)
+let rec generate_mapping_annot (annot : Tast.annotation_def) name = function
+    | [] -> ""
+    | a::q -> if (List.mem a.func_name annot.an_funs || (name = a.func_name)) then "" else "Theorem preservation_"^(a.func_name)^"_"^(annot.an_var)^" : forall (" ^ name ^ " : " ^ name ^") (ether : EtherMap) (msg : Message)" ^ (generate_func_params a.func_params) ^ ", \n let " ^ name ^ "_2 := " ^
+    ( " fst( " ^(a.func_name) ^ " " ^ name ^" ether msg" ^(lemma_func_params a.func_params) ^ ")")
+    ^" in\n (sum_" ^ (annot.an_var) ^ " (IntMap.elements ("^(annot.an_var) ^ " "  ^ name ^ "))) = ( sum_" ^ (annot.an_var) ^ " (IntMap.elements (" ^ (annot.an_var) ^ " " ^ name ^"_2)))" ^
+    ".\nAdmitted.\n\n" ^ (generate_mapping_annot annot name q)
+
+(* Generates the evaluation function for the annotation involving a mapping m, and adds the required Coq modules *)
+let generate_mapping_annot_function name annot m exp =
+    add_required "List"; "Definition mapping_function_"^(annot.an_var) ^ " ( x : Z * " ^ (generate_type m) ^ ") := \n " ^ (generate_expression exp name) ^ ".\n" ^ 
+    "Fixpoint sum_"^(annot.an_var)^" (maplist : list (Z * "^(generate_type m) ^")) := \n match maplist with
+    | nil => 0
+    | a::q => (mapping_function_"^(annot.an_var) ^ " a) + (sum_"^(annot.an_var) ^ " q)\nend.\n"
+
+(** 
+Generates all the functions required to express a property specified as an annotation.
+If the variable v specified in the annotation is a mapping, we first generate the evaluation function specified by calling generate_mapping_annot_function, 
+and then generate all the lemmas needed with generate_mapping_annot.
+If not, we simply generate all the lemmas required by using generate_simple_annot
+**)
+let generate_annot (annot : Tast.annotation_def) name (funs : Tast.function_def list) (state_vars : Tast.variable_def list)  = 
+    match get_annot_var_type annot.an_var state_vars with
+    | TIdent d -> raise (Error ("Custom classes not supported for variables in annotations"))
+    | TMapping (e, m) -> (match annot.an_count_elem with
+        | None -> raise (Error ("Mapping without a count functions for its elements")) 
+        | Some exp -> add_required "Coq.Program.Equality"; add_required "OrderedType"; (generate_mapping_annot_function name annot m exp) ^ (Lemmas.generate_intermediate_lemmas annot.an_var name (generate_type m)) ^ (generate_mapping_annot annot name funs ))
+    | TElem e -> generate_simple_annot annot name funs 
+
+(* Generates all the lemmas corresponding to the annotations by calling generate_annot for all annotations in the contract *)
+let rec generate_annotations (annots : Tast.annotation_def list) name (funs : Tast.function_def list) (svars : Tast.variable_def list) = match annots with
+    | [] -> ""
+    | a::q -> (generate_annot a name funs svars) ^ (generate_annotations q name funs svars) 
+
+(* Generates several helper lemmas to speed up the proof *)
+let generate_lemmas name = Lemmas.generate_helper_lemmas ()
+
+(**
+End of the generation of annotations
+**)
+
+(* Models the send function as well as the ether balances *)
+let create_ethermap_and_send () = 
+    "Definition EtherMap := IntMap.t Z.
+
+Definition get_ether (addr : Z) map : Z :=
+    match (IntMap.find addr map) with
+    | None => 0
+    | Some a => a
+    end.
+
+Definition send addr value map :=
+    if (Z.leb value (get_ether contract_addr map)) then
+        (let map_bis := IntMap.add contract_addr ((get_ether contract_addr map) - value) map in
+        let map_bis := IntMap.add addr ((get_ether addr map_bis) + value) map_bis in
+        (true, map_bis))
+    else (false, map).
+\n"
+
+(* Structure for the message sent by the user to the Ethereum Virtual Machine *)
+let create_message () = 
+    "Record Message := create_message {
+sender : Z;
+value : Z;
+}.\n"
+
+(**
+This function generates the whole contract in Coq.
+It calls all the functions previously defined.
+It first generates the state variables, and store them in the references state_vars and state_list
+It then generates the whole contract, by concatening thei definition for the ether balances, send function, messages,
+generated auxiliary loop functions, functions, and finally lemmas for annotations.
+**)
+let codegen_file (contract : Tast.contract_def) = 
+    List.iter (fun x -> fun_names := (x.func_name)::(!fun_names)) contract.c_funs;
+    let state_decl = generate_state_vars (contract.c_vars) (contract.c_name) in
+    let gen_func = generate_functions (contract.c_funs) (contract.c_name) (contract.c_vars) in
+    let an_func = generate_anonymous_fun (contract.c_anonymousfun) (contract.c_name) in
+    let annot_func = generate_annotations (contract.c_annotations) (contract.c_name) (contract.c_funs) (contract.c_vars) in
+   ("Definition contract_addr := 0.\n") ^ (create_ethermap_and_send ()) ^ (create_message ()) ^ state_decl ^ (create_accessors (contract.c_vars)) ^ (!while_structs) ^ (!while_functions) ^(generate_struct_vars (contract.c_structs) (contract.c_name)) ^ gen_func ^ an_func ^ (generate_lemmas contract.c_name) ^ (Lemmas.generate_extract_sorted_lemma ())^ annot_func
+   
+(* Imports the Coq module that were marked as required *)
+let rec create_required_modules = function
+        | [] -> ""
+        | a::q -> "Require Import " ^ a ^".\n" ^ (create_required_modules q)
+
+(* The entry point of this module. It imports all the required Coq modules by calling create_required_modules, add useful headers
+and finally generates the contract by calling codegen_file *)
+let codegen (file : Tast.file) = 
+    (create_required_modules (!required_modules)) ^ 
+    (if (!open_string) then "Open Scope string_scope.\n" else "") ^
+    ("Open Scope Z_scope.\nInclude BinIntDef.Z.\n") ^
+    ("Module IntMap := FMapList.Make(Z_as_OT).\n") ^
+    (codegen_file (List.hd file.f_contracts))
