Compiler/lemmas.ml
@@ -1,0 +1,339 @@
+module SMap = Map.Make(String)
+let variables = ref [""]
+let typenames = ref SMap.empty
+let count = ref 0
+
+let generate_helper_lemmas () = 
+"Lemma plus_reg_r : forall (n m p : Z), n = m -> p+n= p+m.
+Proof.
+  intros.
+  induction p.
+  auto.
+  rewrite -> H.
+  auto.
+rewrite -> H.
+auto.
+Qed.
+
+Lemma plus_reg_r2 : forall (n m p : Z), n = m -> n+p= m+p.
+Proof.
+  intros.
+  destruct p.
+  rewrite -> H.
+  reflexivity.
+rewrite -> H.
+  reflexivity.
+rewrite -> H.
+  reflexivity.
+Qed.
+
+Lemma plus_reg_l2 : forall (n m p : Z), n+p= m+p -> n = m.
+Proof.
+  intros.
+rewrite <- Z.add_cancel_l with (n := n) (m := m) (p := p).
+rewrite -> Z.add_comm.
+symmetry.
+rewrite -> Z.add_comm.
+symmetry.
+apply H.
+Qed.
+
+Lemma add_0_n : forall (n : Z), n + 0 = n.
+Proof.
+intro.
+now destruct n.
+Qed.
+
+Lemma Zminus_assoc_reverse : forall (n m p : Z), n + m - p = n + (m - p).
+Proof.
+intros.
+assert (m-p = m + -p).
+apply Zplus_minus_eq.
+symmetry.
+apply Zplus_minus.
+rewrite -> H.
+symmetry.
+apply Zplus_minus_eq.
+rewrite -> Zplus_assoc.
+symmetry.
+rewrite -> Z.add_comm.
+rewrite -> Zplus_assoc.
+rewrite -> Z.add_comm.
+apply plus_reg_r.
+rewrite <- Zplus_assoc.
+assert (-p + p = 0).
+destruct p.
+simpl.
+auto.
+simpl.
+apply Z.pos_sub_diag.
+simpl.
+apply Z.pos_sub_diag.
+rewrite -> H0.
+symmetry.
+apply Zplus_0_r_reverse.
+Qed.\n\n"
+
+let generate_extract_sorted_lemma () =
+    let accu = SMap.bindings (!typenames) in
+    let rec aux = function
+        | [] -> ""
+        | (typename, a) :: q ->
+                    
+"
+Lemma extract_Sorted_"^a^" : forall (a b : Z*"^typename^") (l : list (Z * "^typename^")),
+  Sorted.Sorted (IntMap.Raw.PX.ltk (elt:="^typename^")) (a::b::l) -> Sorted.Sorted (IntMap.Raw.PX.ltk (elt:="^typename^")) (b::l).
+Proof.
+  intros.
+  apply Sorted.Sorted_inv in H.
+  apply H.
+Qed. \n\n" ^ aux q in
+    aux accu
+
+let generate_intermediate_lemmas an_var name typename = 
+  if not (List.mem an_var (!variables)) then begin
+      variables := an_var::(!variables);
+      let gen_an_var = "("^an_var^" "^name^"2)" in
+      let sorted_number = try (SMap.find typename (!typenames)) with
+        |Not_found -> (typenames := SMap.add typename (string_of_int (!count)) (!typenames);
+                        count := (!count) + 1;
+                        (string_of_int ((!count) - 1))) in
+      "Lemma update_"^an_var ^" : forall ( "^name ^"2 : "^name^" ) (address : Z) (value : "^typename^"),
+      let balance_map := "^gen_an_var^" in
+      let original_value := match (IntMap.find address "^gen_an_var^") with
+      | None => 0
+      | Some a => mapping_function_"^an_var^"(address, a) end in
+      let balance2 := sum_"^an_var^" (IntMap.elements (IntMap.add address value balance_map)) in
+      (sum_"^an_var^" (IntMap.elements balance_map)) + mapping_function_"^an_var^"(address, value) = balance2 + original_value.
+      Proof.
+      Opaque mapping_function_"^an_var^".
+      intros.
+      case_eq (IntMap.find (elt := "^typename^") address "^gen_an_var^").
+      intro t0.
+      unfold balance2.
+      unfold sum_"^an_var^".
+      simpl.
+      unfold get_"^an_var^".
+      unfold balance_map.
+      destruct "^gen_an_var^".
+      intros.
+      simpl.
+      unfold IntMap.Raw.add.
+      remember (hd this) as a.
+      remember (tl this) as a_bis.
+      dependent induction this.
+      - assert (original_value = 0).
+      simpl in original_value.
+      auto.
+      rewrite -> H0.
+      simpl.
+      symmetry.
+      rewrite -> Z.add_comm.
+      simpl.
+      rewrite -> Z.add_comm.
+      simpl.
+      reflexivity.
+      - simpl.
+      destruct a as (z0, z1).
+      destruct (Z_as_OT.compare).
+      + simpl.
+      assert (IntMap.find (elt := "^typename^") address {| IntMap.this := (z0, z1) :: this; IntMap.sorted := sorted |} = None).
+      unfold IntMap.find.
+      unfold IntMap.Raw.find.
+      simpl.
+      destruct Z_as_OT.compare.
+      reflexivity.
+      unfold Z_as_OT.lt in l.
+      unfold Z_as_OT.eq in e.
+      apply Z_as_OT.lt_not_eq in e.
+      contradiction.
+      apply l.
+      apply Z_as_OT.lt_trans with (x:=z0) (y:=address) (z:=z0) in l0.
+      apply Z_as_OT.lt_not_eq in l0.
+      compute in l0.
+      absurd (z0 = z0).
+      auto.
+      reflexivity.
+      apply l.
+      rewrite -> H0 in H.
+      discriminate.
+      + rewrite <- Z.add_comm.
+      symmetry.
+      rewrite <- Z.add_assoc.
+      apply plus_reg_r.
+      rewrite -> Z.add_comm.
+      assert (original_value = mapping_function_"^an_var^" (z0, z1)).
+      unfold original_value.
+      rewrite -> e.
+      unfold IntMap.find.
+      unfold IntMap.Raw.find.
+      simpl.
+      destruct Z_as_OT.compare.
+      apply Z_as_OT.lt_not_eq in l.
+      absurd (z0 <> z0).
+      auto.
+      apply l.
+      rewrite -> e.
+      reflexivity.
+      apply Z_as_OT.lt_not_eq in l.
+      absurd (z0 <> z0).
+      auto.
+      apply l.
+      rewrite -> H0.
+      reflexivity.
+      + rewrite <- Z.add_assoc.
+      symmetry.
+      rewrite <- Z.add_assoc.
+      apply plus_reg_r.
+      symmetry.
+      assert (Sorted (IntMap.Raw.PX.ltk (elt := "^typename^")) this).
+      induction this.
+      auto.
+      apply extract_Sorted_"^sorted_number^" with (a:=(z0, z1)).
+      apply sorted.
+      assert (original_value = match
+        IntMap.find (elt := "^typename^") address {| IntMap.this := this; IntMap.sorted := H0 |} with
+        | Some a => mapping_function_"^an_var^" (address, a)
+        | None => 0
+        end).
+      unfold original_value.
+      unfold IntMap.find.
+      unfold IntMap.Raw.find.
+      simpl.
+      destruct Z_as_OT.compare.
+      apply Z_as_OT.lt_trans with (x:=address) (y:=z0) (z:=address) in l0.
+      absurd (address < address).
+      auto.
+      apply l0.
+      apply l.
+      rewrite -> e in l.
+      apply Z_as_OT.lt_not_eq in l.
+      absurd (z0 <> z0).
+      auto.
+      apply l.
+      reflexivity.
+      rewrite -> H1.
+      apply IHthis with (sorted := H0) (a := hd this) (a_bis := tl this) (t0:=t0).
+      unfold IntMap.find.
+      unfold IntMap.Raw.find.
+      simpl.
+      unfold IntMap.find in H.
+      unfold IntMap.Raw.find in H.
+      simpl in H.
+      destruct Z_as_OT.compare in H.
+      apply Z_as_OT.lt_trans with (x:=address) (y:=z0) (z:=address) in l0.
+      absurd (address < address).
+      auto.
+      apply l0.
+      apply l.
+      rewrite -> e in l.
+      apply Z_as_OT.lt_not_eq in l.
+      absurd (z0 <> z0).
+      auto.
+      apply l.
+      apply H.
+      reflexivity.
+      reflexivity.
+      - intros.
+      assert (original_value = 0).
+      unfold original_value.
+      rewrite -> H.
+      reflexivity.
+      rewrite -> H0.
+      unfold balance2.
+      unfold balance_map.
+      destruct "^gen_an_var^".
+      simpl.
+      dependent induction this.
+      simpl.
+      symmetry.
+      rewrite -> Z.add_comm.
+      simpl.
+      rewrite -> Z.add_comm.
+      simpl.
+      reflexivity.
+      unfold IntMap.Raw.add.
+      destruct a as (z, t0).
+      destruct Z_as_OT.compare.
+      unfold sum_"^an_var^".
+      rewrite -> Z.add_comm.
+      symmetry.
+      rewrite <- Z.add_assoc.
+      apply plus_reg_r.
+      rewrite -> Z.add_comm.
+      simpl.
+      reflexivity.
+      simpl.
+      assert (original_value = mapping_function_"^an_var^" (z, t0)).
+      unfold original_value.
+      unfold IntMap.find.
+      unfold IntMap.Raw.find.
+      simpl.
+      destruct Z_as_OT.compare.
+      apply Z_as_OT.lt_not_eq in l.
+      rewrite -> e in l.
+      absurd (z <> z).
+      auto.
+      apply l.
+      rewrite -> e.
+      reflexivity.
+      rewrite -> e in l.
+      apply Z_as_OT.lt_not_eq in l.
+      absurd (z <> z).
+      auto.
+      apply l.
+      rewrite -> H0 in H1.
+      rewrite <- H1.
+      simpl.
+      symmetry.
+      rewrite <- Z.add_comm.
+      simpl.
+      rewrite <- Z.add_comm.
+      reflexivity.
+      unfold IntMap.Raw.add in IHthis.
+      unfold sum_"^an_var^".
+      rewrite <- Z.add_assoc.
+      symmetry.
+      rewrite <- Z.add_assoc.
+      symmetry.
+      apply plus_reg_r.
+      unfold sum_"^an_var^" in IHthis.
+      assert (Sorted (IntMap.Raw.PX.ltk (elt := "^typename^")) this).
+      induction this.
+      auto.
+      apply extract_Sorted_"^sorted_number^" with (a:= (z, t0)).
+      apply sorted.
+      apply IHthis with (sorted := H1).
+      unfold IntMap.find.
+      unfold IntMap.Raw.find.
+      simpl.
+      unfold IntMap.find in H.
+      unfold IntMap.Raw.find in H.
+      simpl in H.
+      destruct Z_as_OT.compare in H.
+      apply Z_as_OT.lt_trans with (x:=z) (y:=address) (z:=z) in l.
+      absurd (z<z).
+      auto.
+      apply l.
+      apply l0.
+      discriminate.
+      apply H.
+      assert (IntMap.find (elt := "^typename^") address {| IntMap.this := this; IntMap.sorted := H1 |} = None).
+      unfold IntMap.find.
+      unfold IntMap.Raw.find.
+      simpl.
+      unfold IntMap.find in H.
+      unfold IntMap.Raw.find in H.
+      simpl in H.
+      destruct Z_as_OT.compare in H.
+      apply Z_as_OT.lt_trans with (x:=z) (y:=address) (z:=z) in l.
+      absurd (z<z).
+      auto.
+      apply l.
+      apply l0.
+      discriminate.
+      apply H.
+      rewrite -> H2.
+      reflexivity.
+      Qed.\n"
+  end else ""  
