Compiler/lexer.mll
@@ -1,0 +1,206 @@
+(* Lexer for solidity-coq *)
+
+{
+    open Lexing
+    open Tokens 
+
+    exception LexingError of string
+
+    let keywords = [
+        "_", Underscore;
+        "anonymous", Anonymous;
+        "assembly", Assembly;
+        "break", Break;
+        "constant", Const;
+        "continue", Continue;
+        "contract", Contract;
+        "default", Default;
+        "delete", Delete;
+        "do", Do;
+        "else", Else;
+        "enum", Enum;
+        "event", Event;
+        "external", External;
+        "false", False;
+        "for", For;
+        "function", Function;
+        "if", If;
+        "in", In;
+        "indexed", Indexed;
+        "internal", Internal;
+        "import", Import;
+        "is", Is;
+        "library", Library;
+        "mapping", Mapping;
+        "memory", Memory;
+        "modifier", Modifier;
+        "new", New;
+        "null", Null;
+        "public", Public;
+        "private", Private;
+        "return", Return;
+        "returns", Returns;
+        "storage", Storage;
+        "struct", Struct;
+        "throw", Throw;
+        "true", True;
+        "var", Var;
+        "while", While;
+    ]
+
+    let subdenominations = [
+        "wei", SubWei;
+        "szabo", SubSzabo;
+        "finney", SubFinney;
+        "ether", SubEther;
+        "seconds", SubSeconds;
+        "minutes", SubMinute;
+        "hours", SubHour;
+        "days", SubDays;
+        "weeks", SubWeek;
+        "years", SubYear;
+        "after", After;
+    ]
+
+    let types = [
+        "int", Int;
+        "uint", UInt;
+        "bytes", Bytes;
+        "byte", Byte;
+        "string", String;
+        "address", Address;
+        "bool", Bool;
+        "fixed", Fixed;
+        "ufixed", UFixed;
+     ]
+    
+    let unsupported = ["after"; "break"; "continue"; "default"; "delete"; "do"; "external"; "for"; "import"; "in";  "is"; "library"; "new"; "null"; "days"; "ether"; "finney"; "hours"; "minutes"; "seconds"; "szabo"; "weeks"; "wei"; "years"; "var"]
+
+    let newline lexbuf = 
+        let pos = lexbuf.lex_curr_p in
+        lexbuf.lex_curr_p <- {
+            pos with pos_lnum = pos.pos_lnum + 1;
+            pos_bol = pos.pos_cnum
+        }
+
+    let idOrKeyword s =
+        try List.assoc s keywords with _ -> try List.assoc s subdenominations with | _ -> try List.assoc s types with | _ -> Ident s
+
+    let idOrKeyword_unsupported s =
+        if List.mem s unsupported then raise (LexingError (s ^ " keyword not supported")) else idOrKeyword s
+
+}
+
+    let digit = [ '0' - '9' ]
+    let lowercaseLetter = [ 'a' - 'z' ]
+    let uppercaseLetter = [ 'A' - 'Z' ]
+    let alpha = lowercaseLetter | uppercaseLetter
+    let identStart = '_' | '$' | alpha
+    let ident = identStart (identStart | digit)*
+    let hexa_digit = ['0'-'9' 'a'-'f' 'A'-'F']
+    let integer = '0' | ['1'-'9'] digit* | "0x" hexa_digit+
+    
+    let car = digit | alpha  | ' ' | '!' | '#' | '$' | '%' | '&' | ''' | '('
+    | ')' | '*' | '+' | '-' | ',' | '.' | '/' | ':' | ';' | '<' | '=' | '>' 
+    | '?' | '@' | '[' | ']' | '^' | '_' | '`' | '{' | '|' | '}' | '~' 
+    | "\\\\" | "\\\"" | "\\n" | "\\t"
+    let space = [' ' '\t']
+
+
+rule token = parse 
+    | '\n'                      { newline lexbuf; token lexbuf }
+    | "int" digit+              { Int }
+    | "uint" digit+             { UInt }
+    | "bytes" digit+            { Bytes }
+    | "fixed" digit+ "x" digit+ { Fixed }
+    | "ufixed" digit+ "x" digit+ { UFixed }
+    | (ident as id)             { idOrKeyword_unsupported id }
+    | space+                    { token lexbuf }
+    | "/*"                      { long_comment lexbuf; token lexbuf }
+    | "//"                      { short_comment lexbuf; token lexbuf }
+    | integer as n              { CInt (int_of_string n) }
+    | '@'                       { Atmark }
+    | "\""                      { StringLiteral(strval_double "" lexbuf) }
+    | "\'"                      { StringLiteral(strval_simple "" lexbuf) }
+    | "<"                       { Lt }
+    | "<="                      { Le }
+    | "<<"                      { raise ( LexingError ("character << not supported")) }
+    | "<<="                     { raise ( LexingError ("character <<= not supported")) }
+    | ">"                       { Gt }
+    | ">="                      { Ge }
+    | ">>"                      { raise (LexingError ("character >> not supported")) }
+    | ">>="                     { raise (LexingError ("character >>= not supported")) }
+    | ">>>"                     { raise (LexingError ("character >>> not supported")) }
+    | ">>>="                    { raise (LexingError ("character >>>= not supported")) }
+    | "="                       { Assign }
+    | "=="                      { Equal }
+    | "=>"                      { Arrow }
+    | "!"                       { Not }
+    | "!="                      { NotEqual }
+    | "+"                       { Plus }
+    | "++"                      { Inc }
+    | "+="                      { AssignAdd }
+    | "-"                       { Minus }
+    | "--"                      { Dec }
+    | "-="                      { AssignSub }
+    | "*"                       { Mul }
+    | "**"                      { raise (LexingError ("character ** not supported")) }
+    | "*="                      { AssignMul }
+    | "%"                       { raise (LexingError ("character % not supported")) }
+    | "%="                      { raise (LexingError ("character %= not supported")) }
+    | "/"                       { raise (LexingError ("division not supported")) }
+    | "/="                      { raise (LexingError ("division not supported")) }
+    | "&"                       { raise (LexingError ("BitAnd not supported")) } 
+    | "&&"                      { And }
+    | "&="                      { raise (LexingError ("Bit operations not supported")) }
+    | "|"                       { raise (LexingError ("Bit operations not supported")) }
+    | "|="                      { raise (LexingError ("Bit operations not supported")) }
+    | "||"                      { Or }
+    | "^"                       { raise ( LexingError ("Bit operations not supported")) }
+    | "^="                      { raise ( LexingError ("Bit operations not supported")) }
+    | "."                       { Period }
+    | ":"                       { Colon }
+    | ";"                       { Semicolon }
+    | ","                       { Comma }
+    | "("                       { LParen }
+    | ")"                       { RParen }
+    | "["                       { LBrack }
+    | "]"                       { RBrack }
+    | "{"                       { LBrace }
+    | "}"                       { RBrace }
+    | "?"                       { Conditional }
+    | "~"                       { raise (LexingError ("Bit operations not supported")) }
+    | eof                       { EOF }
+    | _ as c                    { raise (LexingError ("illegal character : " ^ String.make 1 c)) }
+
+and strval_simple s = parse
+    | "\'"              { s }
+    | "\\\\"            { strval_simple (s ^"\\") lexbuf }
+    | "\\\""            { strval_simple (s ^"\"") lexbuf }
+    | "\\n"             { strval_simple (s ^"\n") lexbuf }
+    | "\\t"             { strval_simple (s ^"\t") lexbuf }
+    | "\\"              { raise (LexingError "Invalid Escape Sequence") }  
+    | (car as c)        { strval_simple (s ^c) lexbuf }
+    | eof               { raise (LexingError "Unfinished string") }
+    | _                 { raise (LexingError "Invalid string") }
+
+and strval_double s = parse
+    | "\""              { s }
+    | "\\\\"            { strval_double (s ^"\\") lexbuf }
+    | "\\\""            { strval_double (s ^"\"") lexbuf }
+    | "\\n"             { strval_double (s ^"\n") lexbuf }
+    | "\\t"             { strval_double (s ^"\t") lexbuf }
+    | "\\"              { raise (LexingError "Invalid Escape Sequence") }  
+    | (car as c)        { strval_double (s ^c) lexbuf }
+    | eof               { raise (LexingError "Unfinished string") }
+    | _                 { raise (LexingError "Invalid string") }
+
+and short_comment = parse  
+    | '\n'              { newline lexbuf }
+    | _                 { short_comment lexbuf }
+    | eof               {}
+    
+and long_comment = parse
+    | "*/"              {}
+    | _                 { long_comment lexbuf }
+    | eof               { raise (LexingError "Unclosed comment") }    
