Compiler/main.ml
@@ -1,0 +1,71 @@
+open Format
+open Lexing
+open Passes 
+open Codegen
+
+let parse_only = ref false
+let type_only = ref false
+
+let filename = ref ""
+
+let usage = "usage: solidity-coq [options] file.sol"
+
+let set_var v s = v:=s
+
+let options = ["--parse-only", Arg.Set parse_only, "Stops after parsing the input file";
+               "--type-only", Arg.Set type_only, "Stops after typing the input file"]
+
+let error_loc pos = 
+    let line = pos.pos_lnum in
+    let col = pos.pos_cnum-pos.pos_bol + 1 in
+    eprintf "File \"%s\", line %d, characters %d-%d:\n" !filename line (col-1) col
+
+let localisation2 (pos1, pos2) = 
+    let l = pos1.pos_lnum in
+    let c1 = pos1.pos_cnum - pos1.pos_bol + 1 in
+    let c2 = pos2.pos_cnum - pos2.pos_bol + 1 in
+    eprintf "File \"%s\", line %d, characters %d-%d:\n" !filename l c1 c2
+
+let print_in_file ~file p = 
+    let c = open_out file in
+    let fmt = formatter_of_out_channel c in
+    fprintf fmt "%s" p;
+    pp_print_flush fmt ();
+    close_out c
+
+let () = 
+    Arg.parse options (set_var filename) usage;
+    
+    if !filename = "" then
+        (eprintf "No input file\n@?";
+         exit 2);
+
+    if not (Filename.check_suffix !filename ".sol") then (
+        eprintf "Files must have the .sol extension\n@?";
+        Arg.usage options usage;
+        exit 2);
+
+    let f = open_in !filename in
+    let buf = Lexing.from_channel f in
+    let basename = Filename.chop_suffix (!filename) ".sol" in
+
+    try
+        let p = Parser.file Lexer.token buf in
+        close_in f;
+
+        if not !parse_only then
+        let p = Passes.type_file p in ();
+
+        if not !type_only then
+        let prog = Codegen.codegen p in
+        print_in_file (basename ^".v") prog;
+    with
+        |Lexer.LexingError s ->
+        error_loc (Lexing.lexeme_start_p buf);
+        eprintf "%s\n@?" s;
+        exit 1;
+        |Parser.Error ->
+        error_loc (Lexing.lexeme_start_p buf);
+        eprintf "Syntax error\n@?";
+        exit 1;
+
