Compiler/parser.mly
@@ -1,0 +1,179 @@
+%{
+    open Format
+    open Lexer
+    open Tokens
+    open Ast
+%}
+
+/* Entrypoint */
+%start file
+
+/* Type returned */
+%type <Ast.file> file
+
+%%
+
+file:
+     c_def = contract_definition; EOF { { f_contracts = [c_def] } }
+;
+
+contract_definition:
+    Contract id = Ident LBrace cp = contract_part* RBrace { { c_name = id; 
+    c_parts = cp } }
+    ;
+
+contract_part:
+| e = function_def { FunctionDef e }
+| e = enum_def { EnumDef e}
+| e = struct_def   { StructDef e }
+| e = variable_decl { VariableDecl e }
+| e = event_def    { EventDef e }
+| e = modifier_def { ModifierDef e } 
+| Function; LParen; RParen; b = block_or_empty { AnonymousFun b }
+| Atmark;  e = annotation_def { Annotation e }
+;
+
+enum_def:
+Enum; id = Ident; LBrace ; vals = separated_list(Comma, Ident); RBrace; { { enum_name = id; enum_vals = vals} }
+
+annotation_def:
+   | t = Ident; LParen; id = Ident; RParen { {an_type = t; an_var = id; an_funs = []; an_fname = ""; an_key = ""; an_value = ""; an_count_elem = None } }
+   | t = Ident; LParen; id = Ident; Comma; f = Ident; LParen; key = Ident; Comma; value = Ident; RParen; Assign; e = expression;  RParen { { an_type = t; an_var = id; an_funs = []; an_fname = f; an_key = key; an_value = value; an_count_elem = Some(e) } } 
+
+
+
+visibility_specifier:
+| Public { Public }
+| Private { Private }
+| Internal { Internal }
+;
+
+location_specifier:
+| Memory { Memory }
+| Storage { Storage }
+
+event_def:
+    Event; id = Ident; p = params_list?; Anonymous? ; Semicolon; { { ev_name = id; ev_params = p } }
+;    
+
+%inline rule0:
+| x = visibility_specifier  { VS x }
+| x = location_specifier    { LS x }
+| Const                     { CST }
+;
+
+variable_decl:
+    t = type_name; infos_list = rule0*; id = Ident; e = option(preceded(Assign, expression)); Semicolon; { { v_name = id; v_type = t; v_infos = infos_list; v_expr = e } }
+;
+
+
+struct_def:
+     Struct; id = Ident; LBrace; l = list(variable_decl); RBrace { { s_name = id; s_vars = l } }
+;
+
+function_def:
+    Function; id = Ident; p = params_list; mods = list(Ident); x = rule0*; ret_par = option(preceded(Returns, params_list)); e = block_or_empty; { { func_name = id; func_params = p; func_infos = x; func_ret_params = ret_par; func_insns = e; func_mods = mods } }
+;
+
+modifier_def:
+    Modifier; id=Ident; p=params_list; LBrace; sl = list(statement); Underscore; RBrace; { {mod_name = id; mod_params = p; mod_insns = sl } }
+ ;
+
+block_or_empty:
+| b = block { b }
+| Semicolon { [] }
+;
+
+parameter:
+    t = type_name; Indexed?; id = Ident { (t, id) }
+;
+
+%inline params_list:
+    | LParen; l = separated_list(Comma, parameter); RParen { l }
+    | LParen; t = type_name; RParen { [(t, "Returned_result")] }   
+;
+
+type_name:
+| e = elementary_type_name { TElem (e) }
+| m = mapping { m }
+| id = Ident { TIdent(id) }
+;
+
+elementary_type_name:
+| Int { TEInt }
+| UInt { TEUint }
+| Bytes { TEBytes }
+| Byte { TEByte }
+| String { TEString }
+| Address { TEAddress }
+| Bool { TEBool }
+| Fixed { TEFixed }
+| UFixed { TEUFixed }
+;
+
+mapping:
+    Mapping; LParen; first = elementary_type_name; Arrow; snd = type_name; RParen { TMapping(first, snd) }
+ ;
+ 
+block:
+    LBrace; s = statement*; RBrace { s }
+;
+
+statement:
+| If; LParen; e = expression; RParen; s = statement { SIf (e, s) } %prec If
+| If; LParen; e = expression; RParen; s = statement; Else; s2 = statement { SIfElse(e, s, s2) }
+| While; LParen; e = expression; RParen; LBrace; s = statement*; RBrace { SWhile(e, s) }
+| s = block { SBlock(s) }
+| Return; e = expression?; Semicolon { SReturn (e) }
+| Throw; Semicolon { SThrow }
+| e = expression; Semicolon { SExpr e }
+| v = var_assign; Semicolon { SVarAssign v }
+| d = variable_decl { SVarDecl d }
+;
+
+var_assign:
+| id = Ident; op = assign_op; e = expression;  { VAIdent(op, id, e) }
+| e = expression; Period; id = Ident; op = assign_op; e2 = expression;  { VAField(op, e, id, e2) }
+| id = Ident; exp = nonempty_list(delimited(LBrack, expression, RBrack)); op = assign_op; e = expression;  { VAIdentArray(op, id, exp, e) }
+| e = expression; Period; id = Ident; exp = nonempty_list(delimited(LBrack, expression, RBrack)); op = assign_op; res = expression;  { VAFieldArray(op, e, id, exp, res) }
+;
+
+%inline assign_op:
+| Assign { Assign }
+| AssignAdd { AssignAdd }
+| AssignSub { AssignSub }
+| AssignMul { AssignMul }
+;
+
+expression:
+| i = CInt { EInt i }
+| Minus; i = CInt { EInt (-i) }
+| True { EBool (true) }
+| False { EBool (false) }
+| s = StringLiteral { EStr s }
+| id = Ident { EVar id }
+| e = expression; Period; id = Ident { EFieldVar(e, id) }
+| id = Ident; par = nonempty_list(delimited(LBrack, expression, RBrack)) { EArrayVar (id, par) } 
+| e1 = expression; Conditional; e2 = expression; Colon; e3 = expression { EConditional(e1, e2, e3) } %prec Conditional
+| Not; e = expression { ENot e }
+%prec Not
+| e = expression; Inc { EInc e }
+| e = expression; Dec { EDec e }
+| e1 = expression; op = binop; e2 = expression { EBinOp(op, e1, e2) }
+| id = Ident; LParen; l = separated_list(Comma, expression); RParen { EFunCall(id, l) }
+| e = expression; Period; id = Ident; LParen; l = separated_list(Comma, expression); RParen { EFieldFunCall (e, id, l) }
+;
+
+%inline binop:
+| Lt { OpLt }
+| Le { OpLe }
+| Gt { OpGt }
+| Ge { OpGe }
+| Equal { OpEq }
+| NotEqual { OpNeq }
+| Plus { OpPlus }
+| Minus { OpMinus }
+| Mul { OpMul }
+| And { OpAnd }
+| Or { OpOr}
+;
