Compiler/tast.ml
@@ -1,0 +1,94 @@
+type ident = string
+
+type file = { f_contracts : contract_def list }
+
+and contract_def = { c_name : ident; c_vars : variable_def list; c_structs : struct_def list; c_funs : function_def list; c_anonymousfun : statement list; c_annotations : annotation_def list; c_modifiers : modifier_def list; c_enums : enum_def list }
+
+and enum_def = { enum_name : ident; enum_vals : ident list}
+
+and visibility = 
+| VDefault
+| Public
+| Private
+| Internal
+
+and location_spec = 
+| Memory
+| Storage
+| LDefault
+
+and annotation_def = { an_type : annotation_type; an_var : ident; an_funs : ident list; an_count_elem : expression option}
+
+and annotation_type = 
+| Preservation
+
+and variable_def = { v_name : ident; v_type : type_name; v_visibility : visibility; v_is_const : bool; v_location : location_spec; v_expr : expression option }
+
+and struct_def = { s_name: ident; s_vars : variable_def list }
+ 
+and function_def = { func_name : ident; func_params : (type_name * ident) list; func_vis : visibility; func_ret_params : (type_name * ident) list; func_insns : statement list; func_mods : ident list }
+
+and modifier_def = { mod_name : ident; mod_params : (type_name * ident) list; mod_insns : statement list}
+
+and type_name = 
+| TIdent of ident
+| TMapping of elem_type_name * type_name
+| TElem of elem_type_name
+
+and elem_type_name = 
+| TEInt
+| TEString
+| TEAddress
+| TEBool
+
+and statement =
+| SIf of expression * statement * statement list
+| SIfElse of expression * statement * statement * statement list
+| SWhile of expression * statement list
+| SBlock of statement list
+| SReturn of expression option
+| SThrow
+| SExpr of expression
+| SVarDecl of variable_def
+| SVarAssign of var_assign
+
+and var_assign = 
+| VAIdent of assign_op * ident * expression
+| VAField of assign_op * expression * ident * expression
+| VAIdentArray of assign_op * ident * expression list * expression * type_name
+| VAFieldArray of assign_op * expression * ident * expression list * expression * type_name
+
+and assign_op =
+| Assign
+| AssignAdd
+| AssignSub
+| AssignMul
+
+and expression = 
+| EInt of int
+| EBool of bool
+| EStr of string
+| EVar of ident
+| EFieldVar of expression * ident
+| EArrayVar of ident * expression list
+| EConditional of expression * expression * expression
+| ENot of expression
+| EInc of expression
+| EDec of expression
+| EBinOp of binop * expression * expression
+| EFunCall of ident * expression list
+| EFieldFunCall of expression * ident * expression list
+
+and binop =
+| OpLt
+| OpLe
+| OpGt
+| OpGe
+| OpEq
+| OpNeq
+| OpPlus
+| OpMinus
+| OpMul
+| OpAnd
+| OpOr
+
