Compiler/tokens.mly
@@ -1,0 +1,25 @@
+%token <int> CInt
+%token <string> Ident
+%token <string> StringLiteral
+%token Anonymous Assembly Break Const Continue Contract Default Delete Do Else Enum Event External
+%token False For Function If In Indexed Internal Import Is Library Mapping Memory Modifier New Null
+%token Public Private Return Returns Storage Struct Throw True Var While Underscore
+%token SubWei SubSzabo SubFinney SubEther SubSeconds SubMinute SubHour SubDays SubWeek SubYear After
+%token Int UInt Bytes Byte String Address Bool Fixed UFixed
+%token Lt Le Gt Ge Assign Equal Arrow Not NotEqual Plus Inc AssignAdd Minus Dec AssignSub Mul AssignMul
+%token And Or Period Colon Semicolon Comma LParen RParen LBrack RBrack LBrace RBrace Conditional EOF Atmark
+
+/* Associativity */
+%nonassoc If
+%nonassoc Else
+%nonassoc Conditional
+%nonassoc Not
+%left Or
+%left And
+%left Equal NotEqual
+%left Lt Le Gt Ge
+%left Plus Minus
+%left Mul
+%right Inc Dec
+%left Period
+%%
