MyToken/MyToken.v.d
@@ -1,2 +1,0 @@
-MyToken.vo MyToken.glob MyToken.v.beautified: MyToken.v
-MyToken.vio: MyToken.v
