MyToken/MyToken.v
@@ -1,9 +1,13 @@
+Require Import List.
+Require Import Arith.
 Require Import Nat.
-Require Import Coq.FSets.FMapWeakList.
+Require Import Coq.FSets.FMapList.
 Require Import String.
 Require Import OrderedTypeEx.
+Require Import Coq.Program.Equality.
+Require Import PeanoNat.
 
-Module AddrMap := FMapWeakList.Make(Nat_as_OT).
+Module AddrMap := FMapList.Make(Nat_as_OT).
 Definition MapAddrIntType := AddrMap.t nat.
 
 Definition sender := 0.
@@ -21,19 +25,17 @@ Record MyToken := mytoken {
 Definition create_token (initialSupply:nat) (tokenName:string) (decimalUnits:nat) (tokenSymbol:string) :=
   let startBalance := AddrMap.empty nat in
   let actualBalance := AddrMap.add sender initialSupply startBalance in
-  mytoken tokenName tokenSymbol decimalUnits startBalance (AddrMap.empty MapAddrIntType) (AddrMap.empty MapAddrIntType).
+  mytoken tokenName tokenSymbol decimalUnits actualBalance (AddrMap.empty MapAddrIntType) (AddrMap.empty MapAddrIntType).
+
+Definition get_balance (token : MyToken) (address : nat) :=
+  match AddrMap.find address (balanceOf token) with
+    |None => 0
+    |Some a => a
+  end.
 
 Definition transfer (token:MyToken) (toAddress:nat) (value:nat) :=
-  let obalanceSender := AddrMap.find sender (balanceOf token) in
-  let obalanceReceiver := AddrMap.find toAddress (balanceOf token) in
-  let balanceSender := match obalanceSender with
-    | None =>  0
-    | Some a => a 
-  end in
-  let balanceReceiver := match obalanceReceiver with
-    | None => 0 
-    | Some a => a 
-  end in
+  let balanceSender := get_balance token sender in
+  let balanceReceiver := get_balance token toAddress in
   if (ltb balanceSender value) then token
   else if (ltb (balanceReceiver + value) balanceReceiver) then token 
   else
@@ -41,3 +43,188 @@ Definition transfer (token:MyToken) (toAddress:nat) (value:nat) :=
     let balance := AddrMap.add toAddress (plus balanceReceiver value) balance in
   mytoken (name token) (symbol token) (decimals token) balance (allowance token) (spentAllowance token)
   .
+
+Definition transferFrom (token:MyToken) (fromAddress:nat) (toAddress:nat) (value:nat) := 
+  let obalanceSender := AddrMap.find fromAddress (balanceOf token) in
+  let obalanceReceiver := AddrMap.find toAddress (balanceOf token) in
+  let balanceSender := match obalanceSender with
+    | None => 0
+    | Some a => a
+  end in
+  let balanceReceiver := match obalanceReceiver with
+    | None => 0
+    | Some a => a
+  end in
+  if (ltb balanceSender value) then (token, false)
+  else if (ltb (balanceReceiver + value) balanceReceiver) then (token, false)
+  else 
+  let ospentAllowance := match (AddrMap.find fromAddress (spentAllowance token)) with
+    | None => None
+    | Some a => AddrMap.find sender a
+  end in
+  let currSpentAllowance := match ospentAllowance with
+    | None => 0
+    | Some a => a
+  end in 
+  let oallowance := match (AddrMap.find fromAddress (allowance token)) with
+    | None => None
+    | Some a => AddrMap.find sender a
+  end in
+  let currAllowance := match oallowance with
+    | None => 0
+    | Some a => a
+  end in 
+  if (ltb (currSpentAllowance + value) currAllowance) then (token, false)
+  else 
+    let balance := AddrMap.add fromAddress (minus balanceSender value) (balanceOf token) in
+    let balance := AddrMap.add toAddress (plus balanceReceiver value) balance in
+    let auxSpentAllowance := match (AddrMap.find fromAddress (spentAllowance token)) with
+      | None => AddrMap.empty nat
+      | Some a => a
+    end in
+    let newSpentAllowance := AddrMap.add fromAddress (AddrMap.add sender (currSpentAllowance + value) auxSpentAllowance) (spentAllowance token) in
+    (mytoken (name token) (symbol token) (decimals token) balance (allowance token) newSpentAllowance, true)
+.
+
+Fixpoint sum_onBalance (balance_list : list (nat * nat)) :=
+  match balance_list with
+    | nil => 0
+    | a::q => (snd a) +(sum_onBalance q)
+  end.
+
+Definition totalBalance (token : MyToken) :=
+  sum_onBalance (AddrMap.elements (balanceOf token))
+.
+
+Lemma correct_creation : forall (initial dec : nat ) (name symbol: string), 
+  totalBalance (create_token initial name dec symbol) = initial.
+Proof.
+  intros.
+  unfold totalBalance.
+  unfold balanceOf.
+  simpl.
+  symmetry.
+  apply plus_n_O.
+Qed.
+
+Lemma plus_reg_r : forall (n m p : nat), n = m -> p+n= p+m.
+Proof.
+  intros.
+  auto.
+Qed.
+
+Lemma extract_Sorted : forall (a b : nat*nat) (l : list (nat * nat)),
+  Sorted.Sorted (AddrMap.Raw.PX.ltk (elt:=nat)) (a::b::l) -> Sorted.Sorted (AddrMap.Raw.PX.ltk (elt:=nat)) (b::l).
+Proof.
+  intros.
+  apply Sorted.Sorted_inv in H.
+  apply H.
+Qed.
+
+Lemma update_balance : forall (token : MyToken) (address value : nat),
+  let balance_map := (balanceOf token) in
+  let balance2 := sum_onBalance (AddrMap.elements (AddrMap.add address value balance_map)) in
+  (sum_onBalance (AddrMap.elements balance_map)) + value = balance2 + (get_balance token address).
+Proof.
+  intros.
+  unfold balance2.
+  unfold sum_onBalance.
+  simpl.
+  intros.
+  unfold get_balance.
+  unfold AddrMap.find.
+  replace (balanceOf token) with balance_map.
+  destruct balance_map.
+  simpl.
+  unfold AddrMap.Raw.add.
+  remember (hd this) as a.
+  remember (tl this) as a_bis.
+  dependent induction this.
+-  unfold snd.
+   simpl.
+   elim value.
+  simpl.
+  reflexivity.
+  intros.
+  simpl in |- *.
+  rewrite <- H.
+  reflexivity.
+-  simpl.
+  destruct a.
+  unfold fst.
+  destruct (Nat_as_OT.compare).
+  +simpl.
+  rewrite <- plus_n_O.
+  rewrite -> Nat.add_comm.
+  reflexivity.
+  + simpl.
+  rewrite -> Nat.add_comm.
+  symmetry.
+  rewrite -> plus_assoc_reverse.
+  symmetry.
+  apply plus_reg_r with (p := value) (n := n0 +
+ (fix sum_onBalance (balance_list : list (nat * nat)) : nat :=
+    match balance_list with
+    | nil => 0
+    | a :: q => snd a + sum_onBalance q
+    end) this) (m := (fix sum_onBalance (balance_list : list (nat * nat)) : nat :=
+   match balance_list with
+   | nil => 0
+   | a :: q => snd a + sum_onBalance q
+   end) this + n0).
+  rewrite -> Nat.add_comm.
+  reflexivity.
+  +simpl.
+   rewrite -> plus_assoc_reverse.
+   symmetry.
+   rewrite -> plus_assoc_reverse.
+   apply plus_reg_r with (p := n0) (m := ((fix sum_onBalance (balance_list : list (nat * nat)) : nat :=
+    match balance_list with
+    | nil => 0
+    | a :: q => snd a + sum_onBalance q
+    end) this + value))
+ (n := ((fix sum_onBalance (balance_list : list (nat * nat)) : nat :=
+    match balance_list with
+    | nil => 0
+    | a :: q => snd a + sum_onBalance q
+    end)
+   ((fix add (k : AddrMap.Raw.key) (x : nat) (s : AddrMap.Raw.t nat) {struct s} :
+       AddrMap.Raw.t nat :=
+       match s with
+       | nil => (k, x) :: nil
+       | (k', y) :: l0 =>
+           match Nat_as_OT.compare k k' with
+           | OrderedType.LT _ => (k, x) :: s
+           | OrderedType.EQ _ => (k, x) :: l0
+           | OrderedType.GT _ => (k', y) :: add k x l0
+           end
+       end) address value this) +
+ match AddrMap.Raw.find (elt:=nat) address this with
+ | Some a => a
+ | None => 0
+ end)).
+  induction this.
+  simpl.
+  rewrite <- Nat.add_comm.
+  simpl.
+  rewrite <- Nat.add_comm.
+  simpl.
+  reflexivity.
+  symmetry.
+  apply IHthis with (a0:=hd (a::this)) (a_bis := this).
+  * apply extract_Sorted with (a := (n,n0)).
+    apply sorted.
+  * reflexivity.
+  * reflexivity.
+  - unfold balance_map.
+    reflexivity.
+Qed.
+
+Lemma transfer_preservation : forall (token :MyToken) (toAddress value : nat), 
+  let token2 := transfer token toAddress value in 
+  totalBalance token = totalBalance token2.
+Proof.
+  intros.
+  unfold totalBalance.
+  unfold token2.
+  unfold transfer.
