Auction/Auction.v
@@ -1,0 +1,177 @@
+Require Import Arith.
+Require Import Nat.
+Require Import OrderedTypeEx.
+Require Import Coq.FSets.FMapList.
+Require Import BinInt.
+Require Import BinIntDef.
+Open Scope Z_scope.
+Include BinIntDef.Z.
+Module IntMap := FMapList.Make(Z_as_OT).
+Definition contract_addr := 0.
+
+Definition EtherMap := IntMap.t Z.
+
+Record Message := create_message {
+sender: Z;
+value: Z;
+}.
+
+Definition get_ether (addr : Z) map : Z :=
+  match (IntMap.find addr map) with
+  | None => 0
+  | Some a => a
+  end.
+
+Definition send addr value map := 
+  if (leb value (get_ether contract_addr map)) then 
+    (let map_bis := IntMap.add contract_addr ((get_ether contract_addr map) - value) map in
+    let map_bis := IntMap.add addr ((get_ether addr map_bis) + value) map_bis in
+    (true, map_bis))
+  else (false, map).
+
+Record Auction := create_Auction { 
+bids: IntMap.t (Z);
+isWinner: IntMap.t (bool);
+highestBid: Z;
+}.
+
+Definition get_isWinner (mapping : IntMap.t (bool) ) (a0 : Z) := 
+let m1:= match (IntMap.find a0 mapping)  with
+ | None => false
+ | Some a => a end in 
+m1.
+
+Definition get_money (Auction : Auction) (ether : EtherMap) (msg: Message) :=
+  if (get_isWinner (isWinner Auction) (sender msg)) then 
+  (let (_, new_ether) := send (sender msg) (highestBid Auction) ether in
+    let isWinner := IntMap.add (sender msg) false (isWinner Auction) in
+    (create_Auction (bids Auction) isWinner (highestBid Auction), new_ether))
+  else (Auction, ether).
+
+Require Import Bool.
+
+Lemma test_send : forall (Auction : Auction) (ether : EtherMap) (msg: Message),
+  Is_true (get_isWinner (isWinner Auction) (sender msg)) -> Is_true (ltb 0 (highestBid Auction)) 
+  -> let (_, etherbis) := get_money Auction ether msg in Is_true (ltb (get_ether (sender msg) ether) (get_ether (sender msg) etherbis)).
+Proof.
+intros.
+unfold get_money.
+destruct (get_isWinner (isWinner Auction0) (sender msg)).
+* unfold send.
+  destruct (highestBid Auction0 <=?
+     get_ether contract_addr ether).
+  admit.
+  destruct (get_ether (sender msg) ether <? get_ether (sender msg) ether).
+  trivial.
+  (* This point is impossible : incorrect behaviour *)
+  admit.
+* contradiction.
+Admitted.
+
+
+Definition get_bids (mapping : IntMap.t (Z) ) (a0 : Z) : Z := 
+let m1:= match (IntMap.find a0 mapping)  with
+ | None => 0
+ | Some a => a end in 
+m1.
+
+Definition Auction_constructor (ether: EtherMap) (msg : Message):= 
+let bids := IntMap.empty (Z) in
+let isWinner := IntMap.empty (bool) in
+let highestBid := 0 in
+let highestBid := 0 in 
+let imap1 := match (IntMap.find (sender msg) isWinner) with
+ |None => false
+ | Some a => a end in
+let isWinner := IntMap.add (sender msg) (true)isWinner in
+(create_Auction bids isWinner highestBid).
+
+Definition bid (Auction:Auction) (value:Z) (ether: EtherMap) (msg : Message) := 
+let bids := (bids Auction) in
+let isWinner := (isWinner Auction) in
+let highestBid := (highestBid Auction) in
+let Auction2 := Auction in 
+if (( Z.leb value (get_bids bids  (sender msg)))) then (Auction) 
+else (let imap1 := match (IntMap.find (sender msg) bids) with
+ |None => 0
+ | Some a => a end in
+let bids := IntMap.add (sender msg) (value)bids in
+if (( Z.leb highestBid value)) then (let highestBid := value in 
+let imap1 := match (IntMap.find (sender msg) isWinner) with
+ |None => false
+ | Some a => a end in
+let isWinner := IntMap.add (sender msg) (true)isWinner in
+(create_Auction bids isWinner highestBid)) 
+ else (create_Auction bids isWinner highestBid))
+.
+
+Lemma plus_reg_r : forall (n m p : Z), n = m -> p+n= p+m.
+Proof.
+  intros.
+  induction p.
+  auto.
+  rewrite -> H.
+  auto.
+rewrite -> H.
+auto.
+Qed.
+
+Lemma plus_reg_r2 : forall (n m p : Z), n = m -> n+p= m+p.
+Proof.
+  intros.
+  destruct p.
+  rewrite -> H.
+  reflexivity.
+rewrite -> H.
+  reflexivity.
+rewrite -> H.
+  reflexivity.
+Qed.
+
+Lemma plus_reg_l2 : forall (n m p : Z), n+p= m+p -> n = m.
+Proof.
+  intros.
+rewrite <- Z.add_cancel_l with (n := n) (m := m) (p := p).
+rewrite -> Z.add_comm.
+symmetry.
+rewrite -> Z.add_comm.
+symmetry.
+apply H.
+Qed.
+
+Lemma add_0_n : forall (n : Z), n + 0 = n.
+Proof.
+intro.
+now destruct n.
+Qed.
+
+Lemma Zminus_assoc_reverse : forall (n m p : Z), n + m - p = n + (m - p).
+Proof.
+intros.
+assert (m-p = m + -p).
+apply Zplus_minus_eq.
+symmetry.
+apply Zplus_minus.
+rewrite -> H.
+symmetry.
+apply Zplus_minus_eq.
+rewrite -> Zplus_assoc.
+symmetry.
+rewrite -> Z.add_comm.
+rewrite -> Zplus_assoc.
+rewrite -> Z.add_comm.
+apply plus_reg_r.
+rewrite <- Zplus_assoc.
+assert (-p + p = 0).
+destruct p.
+simpl.
+auto.
+simpl.
+apply Z.pos_sub_diag.
+simpl.
+apply Z.pos_sub_diag.
+rewrite -> H0.
+symmetry.
+apply Zplus_0_r_reverse.
+Qed.
+
