Ballot/Ballot.v
@@ -1,0 +1,469 @@
+Require Import List.
+Require Import OrderedType.
+Require Import Coq.Program.Equality.
+Require Import Arith.
+Require Import Nat.
+Require Import OrderedTypeEx.
+Require Import Coq.FSets.FMapList.
+Require Import BinInt.
+Require Import BinIntDef.
+Open Scope Z_scope.
+Include BinIntDef.Z.
+Module IntMap := FMapList.Make(Z_as_OT).
+Definition sender := 0.
+Record Ballot := create_Ballot { 
+voteCounts: IntMap.t (Z);
+delegations: IntMap.t (Z);
+votes: IntMap.t (Z);
+voted: IntMap.t (bool);
+voterWeight: IntMap.t (Z);
+numProposals: Z;
+chairperson: Z;
+}.
+Definition get_voteCounts (mapping : IntMap.t (Z) ) (a0 : Z) := 
+let m1:= match (IntMap.find a0 mapping)  with
+ | None => 0
+ | Some a => a end in 
+m1.
+Definition get_delegations (mapping : IntMap.t (Z) ) (a0 : Z) := 
+let m1:= match (IntMap.find a0 mapping)  with
+ | None => 0
+ | Some a => a end in 
+m1.
+Definition get_votes (mapping : IntMap.t (Z) ) (a0 : Z) := 
+let m1:= match (IntMap.find a0 mapping)  with
+ | None => 0
+ | Some a => a end in 
+m1.
+Definition get_voted (mapping : IntMap.t (bool) ) (a0 : Z) := 
+let m1:= match (IntMap.find a0 mapping)  with
+ | None => false
+ | Some a => a end in 
+m1.
+Definition get_voterWeight (mapping : IntMap.t (Z) ) (a0 : Z) := 
+let m1:= match (IntMap.find a0 mapping)  with
+ | None => 0
+ | Some a => a end in 
+m1.
+Definition Ballot_constructor(_numProposals:Z)  := 
+let voteCounts := IntMap.empty (Z) in
+let delegations := IntMap.empty (Z) in
+let votes := IntMap.empty (Z) in
+let voted := IntMap.empty (bool) in
+let voterWeight := IntMap.empty (Z) in
+let numProposals := 0 in
+let chairperson := 0 in
+let chairperson := sender in 
+let numProposals := _numProposals in 
+(create_Ballot voteCounts delegations votes voted voterWeight numProposals chairperson).
+Definition giveRightToVote (Ballot:Ballot) (voter:Z)  := 
+let voteCounts := (voteCounts Ballot) in
+let delegations := (delegations Ballot) in
+let votes := (votes Ballot) in
+let voted := (voted Ballot) in
+let voterWeight := (voterWeight Ballot) in
+let numProposals := (numProposals Ballot) in
+let chairperson := (chairperson Ballot) in
+let Ballot2 := Ballot in 
+if ((get_voted voted  (voter))) then ((create_Ballot voteCounts delegations votes voted voterWeight numProposals chairperson)) 
+ else let imap1 := match (IntMap.find voter voterWeight) with
+ |None => 0
+ | Some a => a end in
+let voterWeight := IntMap.add voter (1)voterWeight in
+(create_Ballot voteCounts delegations votes voted voterWeight numProposals chairperson).
+Definition delegate (Ballot:Ballot) (to:Z)  := 
+let voteCounts := (voteCounts Ballot) in
+let delegations := (delegations Ballot) in
+let votes := (votes Ballot) in
+let voted := (voted Ballot) in
+let voterWeight := (voterWeight Ballot) in
+let numProposals := (numProposals Ballot) in
+let chairperson := (chairperson Ballot) in
+let Ballot2 := Ballot in 
+if ((get_voted voted  (sender))) then ((create_Ballot voteCounts delegations votes voted voterWeight numProposals chairperson)) 
+ else if (( eqb to sender)) then ((create_Ballot voteCounts delegations votes voted voterWeight numProposals chairperson)) 
+ else let imap1 := match (IntMap.find sender voted) with
+ |None => false
+ | Some a => a end in
+let voted := IntMap.add sender (true)voted in
+let imap1 := match (IntMap.find sender delegations) with
+ |None => 0
+ | Some a => a end in
+let delegations := IntMap.add sender (to)delegations in
+if ((get_voted voted  (to))) then (let imap1 := match (IntMap.find (get_votes votes  (to)) voteCounts) with
+ |None => 0
+ | Some a => a end in
+let voteCounts := IntMap.add (get_votes votes  (to)) (((get_voteCounts voteCounts  ((get_votes votes  (to)))) + (get_voterWeight voterWeight  (sender))))voteCounts in
+(create_Ballot voteCounts delegations votes voted voterWeight numProposals chairperson)) 
+else (let imap1 := match (IntMap.find to voterWeight) with
+ |None => 0
+ | Some a => a end in
+let voterWeight := IntMap.add to (((get_voterWeight voterWeight  (to)) + (get_voterWeight voterWeight  (sender))))voterWeight in
+let imap1 := match (IntMap.find sender voterWeight) with
+ |None => 0
+ | Some a => a end in
+let voterWeight := IntMap.add sender (0)voterWeight in
+(create_Ballot voteCounts delegations votes voted voterWeight numProposals chairperson))
+.
+Definition vote (Ballot:Ballot) (proposal:Z)  := 
+let voteCounts := (voteCounts Ballot) in
+let delegations := (delegations Ballot) in
+let votes := (votes Ballot) in
+let voted := (voted Ballot) in
+let voterWeight := (voterWeight Ballot) in
+let numProposals := (numProposals Ballot) in
+let chairperson := (chairperson Ballot) in
+let Ballot2 := Ballot in 
+if (( orb (get_voted voted  (sender)) ( ltb numProposals proposal))) then ((create_Ballot voteCounts delegations votes voted voterWeight numProposals chairperson)) 
+ else let imap1 := match (IntMap.find sender voted) with
+ |None => false
+ | Some a => a end in
+let voted := IntMap.add sender (true)voted in
+let imap1 := match (IntMap.find sender votes) with
+ |None => 0
+ | Some a => a end in
+let votes := IntMap.add sender (proposal)votes in
+let imap1 := match (IntMap.find proposal voteCounts) with
+ |None => 0
+ | Some a => a end in
+let voteCounts := IntMap.add proposal (((get_voteCounts voteCounts  (proposal)) + (get_voterWeight voterWeight  (sender))))voteCounts in
+(create_Ballot voteCounts delegations votes voted voterWeight numProposals chairperson).
+Lemma plus_reg_r : forall (n m p : Z), n = m -> p+n= p+m.
+Proof.
+  intros.
+  induction p.
+  auto.
+  rewrite -> H.
+  auto.
+rewrite -> H.
+auto.
+Qed.
+
+Lemma plus_reg_r2 : forall (n m p : Z), n = m -> n+p= m+p.
+Proof.
+  intros.
+  destruct p.
+  rewrite -> H.
+  reflexivity.
+rewrite -> H.
+  reflexivity.
+rewrite -> H.
+  reflexivity.
+Qed.
+
+Lemma plus_reg_l2 : forall (n m p : Z), n+p= m+p -> n = m.
+Proof.
+  intros.
+rewrite <- Z.add_cancel_l with (n := n) (m := m) (p := p).
+rewrite -> Z.add_comm.
+symmetry.
+rewrite -> Z.add_comm.
+symmetry.
+apply H.
+Qed.
+
+Lemma add_0_n : forall (n : Z), n + 0 = n.
+Proof.
+intro.
+now destruct n.
+Qed.
+
+Lemma Zminus_assoc_reverse : forall (n m p : Z), n + m - p = n + (m - p).
+Proof.
+intros.
+assert (m-p = m + -p).
+apply Zplus_minus_eq.
+symmetry.
+apply Zplus_minus.
+rewrite -> H.
+symmetry.
+apply Zplus_minus_eq.
+rewrite -> Zplus_assoc.
+symmetry.
+rewrite -> Z.add_comm.
+rewrite -> Zplus_assoc.
+rewrite -> Z.add_comm.
+apply plus_reg_r.
+rewrite <- Zplus_assoc.
+assert (-p + p = 0).
+destruct p.
+simpl.
+auto.
+simpl.
+apply Z.pos_sub_diag.
+simpl.
+apply Z.pos_sub_diag.
+rewrite -> H0.
+symmetry.
+apply Zplus_0_r_reverse.
+Qed.
+
+
+Lemma extract_Sorted_0 : forall (a b : Z*Z) (l : list (Z * Z)),
+  Sorted.Sorted (IntMap.Raw.PX.ltk (elt:=Z)) (a::b::l) -> Sorted.Sorted (IntMap.Raw.PX.ltk (elt:=Z)) (b::l).
+Proof.
+  intros.
+  apply Sorted.Sorted_inv in H.
+  apply H.
+Qed. 
+
+Definition mapping_function_voterWeight ( x : Z * Z) := 
+ (snd (x)).
+Fixpoint sum_voterWeight (maplist : list (Z * Z)) := 
+ match maplist with
+    | nil => 0
+    | a::q => (mapping_function_voterWeight a) + (sum_voterWeight q)
+end.
+Lemma update_voterWeight : forall ( Ballot2 : Ballot ) (address : Z) (value : Z),
+      let balance_map := (voterWeight Ballot2) in
+      let original_value := match (IntMap.find address (voterWeight Ballot2)) with
+      | None => 0
+      | Some a => mapping_function_voterWeight(address, a) end in
+      let balance2 := sum_voterWeight (IntMap.elements (IntMap.add address value balance_map)) in
+      (sum_voterWeight (IntMap.elements balance_map)) + mapping_function_voterWeight(address, value) = balance2 + original_value.
+      Proof.
+      Opaque mapping_function_voterWeight.
+      intros.
+      case_eq (IntMap.find (elt := Z) address (voterWeight Ballot2)).
+      intro t0.
+      unfold balance2.
+      unfold sum_voterWeight.
+      simpl.
+      unfold get_voterWeight.
+      unfold balance_map.
+      destruct (voterWeight Ballot2).
+      intros.
+      simpl.
+      unfold IntMap.Raw.add.
+      remember (hd this) as a.
+      remember (tl this) as a_bis.
+      dependent induction this.
+      - assert (original_value = 0).
+      simpl in original_value.
+      auto.
+      rewrite -> H0.
+      simpl.
+      symmetry.
+      rewrite -> Z.add_comm.
+      simpl.
+      rewrite -> Z.add_comm.
+      simpl.
+      reflexivity.
+      - simpl.
+      destruct a as (z0, z1).
+      destruct (Z_as_OT.compare).
+      + simpl.
+      assert (IntMap.find (elt := Z) address {| IntMap.this := (z0, z1) :: this; IntMap.sorted := sorted |} = None).
+      unfold IntMap.find.
+      unfold IntMap.Raw.find.
+      simpl.
+      destruct Z_as_OT.compare.
+      reflexivity.
+      unfold Z_as_OT.lt in l.
+      unfold Z_as_OT.eq in e.
+      apply Z_as_OT.lt_not_eq in e.
+      contradiction.
+      apply l.
+      apply Z_as_OT.lt_trans with (x:=z0) (y:=address) (z:=z0) in l0.
+      apply Z_as_OT.lt_not_eq in l0.
+      compute in l0.
+      absurd (z0 = z0).
+      auto.
+      reflexivity.
+      apply l.
+      rewrite -> H0 in H.
+      discriminate.
+      + rewrite <- Z.add_comm.
+      symmetry.
+      rewrite <- Z.add_assoc.
+      apply plus_reg_r.
+      rewrite -> Z.add_comm.
+      assert (original_value = mapping_function_voterWeight (z0, z1)).
+      unfold original_value.
+      rewrite -> e.
+      unfold IntMap.find.
+      unfold IntMap.Raw.find.
+      simpl.
+      destruct Z_as_OT.compare.
+      apply Z_as_OT.lt_not_eq in l.
+      absurd (z0 <> z0).
+      auto.
+      apply l.
+      rewrite -> e.
+      reflexivity.
+      apply Z_as_OT.lt_not_eq in l.
+      absurd (z0 <> z0).
+      auto.
+      apply l.
+      rewrite -> H0.
+      reflexivity.
+      + rewrite <- Z.add_assoc.
+      symmetry.
+      rewrite <- Z.add_assoc.
+      apply plus_reg_r.
+      symmetry.
+      assert (Sorted (IntMap.Raw.PX.ltk (elt := Z)) this).
+      induction this.
+      auto.
+      apply extract_Sorted_0 with (a:=(z0, z1)).
+      apply sorted.
+      assert (original_value = match
+        IntMap.find (elt := Z) address {| IntMap.this := this; IntMap.sorted := H0 |} with
+        | Some a => mapping_function_voterWeight (address, a)
+        | None => 0
+        end).
+      unfold original_value.
+      unfold IntMap.find.
+      unfold IntMap.Raw.find.
+      simpl.
+      destruct Z_as_OT.compare.
+      apply Z_as_OT.lt_trans with (x:=address) (y:=z0) (z:=address) in l0.
+      absurd (address < address).
+      auto.
+      apply l0.
+      apply l.
+      rewrite -> e in l.
+      apply Z_as_OT.lt_not_eq in l.
+      absurd (z0 <> z0).
+      auto.
+      apply l.
+      reflexivity.
+      rewrite -> H1.
+      apply IHthis with (sorted := H0) (a := hd this) (a_bis := tl this) (t0:=t0).
+      unfold IntMap.find.
+      unfold IntMap.Raw.find.
+      simpl.
+      unfold IntMap.find in H.
+      unfold IntMap.Raw.find in H.
+      simpl in H.
+      destruct Z_as_OT.compare in H.
+      apply Z_as_OT.lt_trans with (x:=address) (y:=z0) (z:=address) in l0.
+      absurd (address < address).
+      auto.
+      apply l0.
+      apply l.
+      rewrite -> e in l.
+      apply Z_as_OT.lt_not_eq in l.
+      absurd (z0 <> z0).
+      auto.
+      apply l.
+      apply H.
+      reflexivity.
+      reflexivity.
+      - intros.
+      assert (original_value = 0).
+      unfold original_value.
+      rewrite -> H.
+      reflexivity.
+      rewrite -> H0.
+      unfold balance2.
+      unfold balance_map.
+      destruct (voterWeight Ballot2).
+      simpl.
+      dependent induction this.
+      simpl.
+      symmetry.
+      rewrite -> Z.add_comm.
+      simpl.
+      rewrite -> Z.add_comm.
+      simpl.
+      reflexivity.
+      unfold IntMap.Raw.add.
+      destruct a as (z, t0).
+      destruct Z_as_OT.compare.
+      unfold sum_voterWeight.
+      rewrite -> Z.add_comm.
+      symmetry.
+      rewrite <- Z.add_assoc.
+      apply plus_reg_r.
+      rewrite -> Z.add_comm.
+      simpl.
+      reflexivity.
+      simpl.
+      assert (original_value = mapping_function_voterWeight (z, t0)).
+      unfold original_value.
+      unfold IntMap.find.
+      unfold IntMap.Raw.find.
+      simpl.
+      destruct Z_as_OT.compare.
+      apply Z_as_OT.lt_not_eq in l.
+      rewrite -> e in l.
+      absurd (z <> z).
+      auto.
+      apply l.
+      rewrite -> e.
+      reflexivity.
+      rewrite -> e in l.
+      apply Z_as_OT.lt_not_eq in l.
+      absurd (z <> z).
+      auto.
+      apply l.
+      rewrite -> H0 in H1.
+      rewrite <- H1.
+      simpl.
+      symmetry.
+      rewrite <- Z.add_comm.
+      simpl.
+      rewrite <- Z.add_comm.
+      reflexivity.
+      unfold IntMap.Raw.add in IHthis.
+      unfold sum_voterWeight.
+      rewrite <- Z.add_assoc.
+      symmetry.
+      rewrite <- Z.add_assoc.
+      symmetry.
+      apply plus_reg_r.
+      unfold sum_voterWeight in IHthis.
+      assert (Sorted (IntMap.Raw.PX.ltk (elt := Z)) this).
+      induction this.
+      auto.
+      apply extract_Sorted_0 with (a:= (z, t0)).
+      apply sorted.
+      apply IHthis with (sorted := H1).
+      unfold IntMap.find.
+      unfold IntMap.Raw.find.
+      simpl.
+      unfold IntMap.find in H.
+      unfold IntMap.Raw.find in H.
+      simpl in H.
+      destruct Z_as_OT.compare in H.
+      apply Z_as_OT.lt_trans with (x:=z) (y:=address) (z:=z) in l.
+      absurd (z<z).
+      auto.
+      apply l.
+      apply l0.
+      discriminate.
+      apply H.
+      assert (IntMap.find (elt := Z) address {| IntMap.this := this; IntMap.sorted := H1 |} = None).
+      unfold IntMap.find.
+      unfold IntMap.Raw.find.
+      simpl.
+      unfold IntMap.find in H.
+      unfold IntMap.Raw.find in H.
+      simpl in H.
+      destruct Z_as_OT.compare in H.
+      apply Z_as_OT.lt_trans with (x:=z) (y:=address) (z:=z) in l.
+      absurd (z<z).
+      auto.
+      apply l.
+      apply l0.
+      discriminate.
+      apply H.
+      rewrite -> H2.
+      reflexivity.
+      Qed.
+Lemma preservation_vote_voterWeight : forall (Ballot : Ballot) (proposal:Z) , 
+ let Ballot_2 := vote Ballot proposal in
+ (sum_voterWeight (IntMap.elements (voterWeight Ballot))) = ( sum_voterWeight (IntMap.elements (voterWeight Ballot_2))).
+Admitted.
+
+Lemma preservation_delegate_voterWeight : forall (Ballot : Ballot) (to:Z) , 
+ let Ballot_2 := delegate Ballot to in
+ (sum_voterWeight (IntMap.elements (voterWeight Ballot))) = ( sum_voterWeight (IntMap.elements (voterWeight Ballot_2))).
+Admitted.
+
+Lemma preservation_giveRightToVote_voterWeight : forall (Ballot : Ballot) (voter:Z) , 
+ let Ballot_2 := giveRightToVote Ballot voter in
+ (sum_voterWeight (IntMap.elements (voterWeight Ballot))) = ( sum_voterWeight (IntMap.elements (voterWeight Ballot_2))).
+Admitted.
+
