README.md
@@ -2,4 +2,25 @@
 
 The goal of this project is to use Coq to model smart contracts written in [Solidity](https://www.ethereum.org/token), developped by the [Ethereum fondation](https://www.ethereum.org).
 
-For the moment, we're translating ourselves the programs into Coq.
+A compiler from Solidity to Coq can be found in the Compiler folder. It requires OCaml and Menhir.
+To install it, run 'make'.
+Then, run 'solidity-coq' on any solidity file with a .sol extension.
+
+A Docker image is also provided, with this compiler already installed. Just run sh launch\_docker.sh, and type 'cd /home/Compiler'
+
+This compiler assumes that the Solidity program given as an input is a valid Solidity program.
+
+The grammar supported is defined in solidity-grammar-subset. 
+The main Solidity features which are not supported are the following :
+* Several contracts, and inheritance
+* Enums structures
+
+Several solidity programs can be found in the Compiler/tests folder, extracted from [Etherscrape](http://etherscrape.com/solidity/download). Programs correct according to Solidity are in the success folder, programs failing solidity compilation are in the fail folder.
+
+
+It is possible to add annotations in Solidity contracts to automatically generate lemmas and theoremes to ensure these properties. At the moment, we only support annotations expressing preservation properties.
+To express that a state variable `v` is preservered throughout any execution of the contract, one has to write the annotation
+`@preservation(v)`
+It is also possible to express that the sum of an evaluation function on all pairs (key, value) in a mapping is preserved. For instance, if we have a mapping `balance` containing the amount of money each user owns, we can write the annotation `@preservation(balance, fun(key, value) = value)` to express that the sum of all values stored in the mapping, i.e. the total amount of money remains constant.
+
+Examples of the compilation from Coq to Solidity can be found in the Ballot, Auction and MyToken folders.
